<?xml version="1.0"?>
<rdf:RDF xmlns="http://www.w3.org/ns/ssn/"
     xml:base="http://www.w3.org/ns/ssn/"
     xmlns:owl="http://www.w3.org/2002/07/owl#"
     xmlns:rdf="http://www.w3.org/1999/02/22-rdf-syntax-ns#"
     xmlns:ssn="http://www.w3.org/ns/ssn/"
     xmlns:xml="http://www.w3.org/XML/1998/namespace"
     xmlns:xsd="http://www.w3.org/2001/XMLSchema#"
     xmlns:foaf="http://xmlns.com/foaf/0.1/"
     xmlns:rdfs="http://www.w3.org/2000/01/rdf-schema#"
     xmlns:skos="http://www.w3.org/2004/02/skos/core#"
     xmlns:sosa="http://www.w3.org/ns/sosa/"
     xmlns:time="http://www.w3.org/2006/time#"
     xmlns:vann="http://purl.org/vocab/vann/"
     xmlns:voaf="http://purl.org/vocommons/voaf#"
     xmlns:schema="http://schema.org/"
     xmlns:dcterms="http://purl.org/dc/terms/"
     xmlns:ssn-ext="http://www.w3.org/TR/vocab-ssn-ext/"
     xmlns:systems="http://www.w3.org/ns/ssn/systems/"
     xmlns:sampling="http://www.w3.org/ns/sosa/sampling/">
    <owl:Ontology rdf:about="http://www.w3.org/ns/ssn/">
        <owl:imports rdf:resource="http://www.w3.org/ns/sosa/"/>
        <dcterms:created rdf:datatype="http://www.w3.org/2001/XMLSchema#date">2017-04-17</dcterms:created>
        <dcterms:creator>
            <rdf:Description>
                <rdf:type rdf:resource="http://xmlns.com/foaf/0.1/Agent"/>
                <foaf:name xml:lang="en">W3C/OGC Spatial Data on the Web Working Group</foaf:name>
            </rdf:Description>
        </dcterms:creator>
        <dcterms:license rdf:resource="http://www.opengeospatial.org/ogc/Software"/>
        <dcterms:license rdf:resource="http://www.w3.org/Consortium/Legal/2015/copyright-software-and-document"/>
        <vann:preferredNamespaceUri>http://www.w3.org/ns/ssn/</vann:preferredNamespaceUri>
        <rdfs:comment xml:lang="en">Please report any errors to the W3C Spatial Data on the Web Working Group via the SDW WG Public List public-sdw-wg@w3.org</rdfs:comment>
        <rdfs:seeAlso rdf:resource="https://www.w3.org/2015/spatial/wiki/Semantic_Sensor_Network_Ontology"/>
        <owl:versionInfo xml:lang="en">New modular version of the SSN ontology. 

This ontology was originally developed in 2009-2011 by the W3C Semantic Sensor Networks Incubator Group (SSN-XG). For more information on the group&apos;s activities see: http://www.w3.org/2005/Incubator/ssn/. The ontology was revised and modularized in 2015-2017 by the W3C/OGC Spatial Data on the Web Working Group, see: https://www.w3.org/2015/spatial/wiki/Semantic_Sensor_Network_Ontology. 

In particular, (a) the scope is extended to include actuation and sampling; (b) the core concepts and properties are factored out into the SOSA ontology. The SSN ontology imports SOSA and adds formal axiomatization consistent with the text definitions in SOSA, and adds classes and properties to accommodate the scope of the original SSN ontology. </owl:versionInfo>
    </owl:Ontology>
    


    <!-- 
    ///////////////////////////////////////////////////////////////////////////////////////
    //
    // Annotation properties
    //
    ///////////////////////////////////////////////////////////////////////////////////////
     -->

    


    <!-- http://purl.org/dc/terms/created -->

    <owl:AnnotationProperty rdf:about="http://purl.org/dc/terms/created"/>
    


    <!-- http://purl.org/dc/terms/creator -->

    <owl:AnnotationProperty rdf:about="http://purl.org/dc/terms/creator"/>
    


    <!-- http://purl.org/dc/terms/description -->

    <owl:AnnotationProperty rdf:about="http://purl.org/dc/terms/description"/>
    


    <!-- http://purl.org/dc/terms/license -->

    <owl:AnnotationProperty rdf:about="http://purl.org/dc/terms/license"/>
    


    <!-- http://purl.org/dc/terms/rights -->

    <owl:AnnotationProperty rdf:about="http://purl.org/dc/terms/rights"/>
    


    <!-- http://purl.org/dc/terms/title -->

    <owl:AnnotationProperty rdf:about="http://purl.org/dc/terms/title"/>
    


    <!-- http://purl.org/vocab/vann/preferredNamespacePrefix -->

    <owl:AnnotationProperty rdf:about="http://purl.org/vocab/vann/preferredNamespacePrefix"/>
    


    <!-- http://purl.org/vocab/vann/preferredNamespaceUri -->

    <owl:AnnotationProperty rdf:about="http://purl.org/vocab/vann/preferredNamespaceUri"/>
    


    <!-- http://www.w3.org/2004/02/skos/core#definition -->

    <owl:AnnotationProperty rdf:about="http://www.w3.org/2004/02/skos/core#definition"/>
    


    <!-- http://www.w3.org/2004/02/skos/core#example -->

    <owl:AnnotationProperty rdf:about="http://www.w3.org/2004/02/skos/core#example"/>
    


    <!-- http://xmlns.com/foaf/0.1/name -->

    <owl:AnnotationProperty rdf:about="http://xmlns.com/foaf/0.1/name"/>
    


    <!-- 
    ///////////////////////////////////////////////////////////////////////////////////////
    //
    // Object Properties
    //
    ///////////////////////////////////////////////////////////////////////////////////////
     -->

    


    <!-- http://www.w3.org/TR/vocab-ssn-ext/hasMember -->

    <owl:ObjectProperty rdf:about="http://www.w3.org/TR/vocab-ssn-ext/hasMember">
        <rdfs:domain rdf:resource="http://www.w3.org/TR/vocab-ssn-ext/ObservationCollection"/>
        <rdfs:range rdf:resource="http://www.w3.org/TR/vocab-ssn-ext/ObservationCollection"/>
        <rdfs:range rdf:resource="http://www.w3.org/ns/sosa/Observation"/>
        <rdfs:comment>Link to a member of a collection of observations that share the same value for one or more of the characteristic properties.</rdfs:comment>
    </owl:ObjectProperty>
    


    <!-- http://www.w3.org/TR/vocab-ssn-ext/hasUltimateFeatureOfInterest -->

    <owl:ObjectProperty rdf:about="http://www.w3.org/TR/vocab-ssn-ext/hasUltimateFeatureOfInterest">
        <rdfs:range rdf:resource="http://www.w3.org/ns/sosa/FeatureOfInterest"/>
        <rdfs:comment>Link to the ultimate feature of interest of an observation or act of sampling. This is useful when the proximate feature of interest is a sample of the ultimate feature of interest, directly or transitively.</rdfs:comment>
    </owl:ObjectProperty>
    


    <!-- http://www.w3.org/ns/sosa/actsOnProperty -->

    <rdf:Description rdf:about="http://www.w3.org/ns/sosa/actsOnProperty">
        <rdfs:domain rdf:resource="http://www.w3.org/ns/sosa/Actuation"/>
        <rdfs:range rdf:resource="http://www.w3.org/ns/sosa/ActuatableProperty"/>
        <rdfs:isDefinedBy rdf:resource="http://www.w3.org/ns/sosa/"/>
    </rdf:Description>
    


    <!-- http://www.w3.org/ns/sosa/hasFeatureOfInterest -->

    <rdf:Description rdf:about="http://www.w3.org/ns/sosa/hasFeatureOfInterest">
        <rdfs:domain rdf:resource="http://www.w3.org/ns/sosa/Actuation"/>
        <rdfs:domain rdf:resource="http://www.w3.org/ns/sosa/Observation"/>
        <rdfs:domain rdf:resource="http://www.w3.org/ns/sosa/Sampling"/>
        <rdfs:range rdf:resource="http://www.w3.org/ns/sosa/FeatureOfInterest"/>
        <rdfs:range rdf:resource="http://www.w3.org/ns/sosa/Sample"/>
        <rdfs:isDefinedBy rdf:resource="http://www.w3.org/ns/sosa/"/>
    </rdf:Description>
    


    <!-- http://www.w3.org/ns/sosa/hasResult -->

    <rdf:Description rdf:about="http://www.w3.org/ns/sosa/hasResult">
        <rdfs:domain rdf:resource="http://www.w3.org/ns/sosa/Actuation"/>
        <rdfs:domain rdf:resource="http://www.w3.org/ns/sosa/Observation"/>
        <rdfs:domain rdf:resource="http://www.w3.org/ns/sosa/Sampling"/>
        <rdfs:range rdf:resource="http://www.w3.org/ns/sosa/Result"/>
        <rdfs:range rdf:resource="http://www.w3.org/ns/sosa/Sample"/>
        <rdfs:isDefinedBy rdf:resource="http://www.w3.org/ns/sosa/"/>
    </rdf:Description>
    


    <!-- http://www.w3.org/ns/sosa/hasSample -->

    <owl:ObjectProperty rdf:about="http://www.w3.org/ns/sosa/hasSample">
        <rdf:type rdf:resource="http://www.w3.org/2002/07/owl#InverseFunctionalProperty"/>
        <rdfs:domain rdf:resource="http://www.w3.org/ns/sosa/FeatureOfInterest"/>
        <rdfs:range rdf:resource="http://www.w3.org/ns/sosa/Sample"/>
        <rdfs:isDefinedBy rdf:resource="http://www.w3.org/ns/sosa/"/>
    </owl:ObjectProperty>
    


    <!-- http://www.w3.org/ns/sosa/hosts -->

    <rdf:Description rdf:about="http://www.w3.org/ns/sosa/hosts">
        <rdfs:domain rdf:resource="http://www.w3.org/ns/sosa/Platform"/>
        <rdfs:range rdf:resource="http://www.w3.org/ns/sosa/Actuator"/>
        <rdfs:range rdf:resource="http://www.w3.org/ns/sosa/Platform"/>
        <rdfs:range rdf:resource="http://www.w3.org/ns/sosa/Sampler"/>
        <rdfs:range rdf:resource="http://www.w3.org/ns/sosa/Sensor"/>
        <owl:propertyChainAxiom rdf:parseType="Collection">
            <rdf:Description rdf:about="http://www.w3.org/ns/ssn/inDeployment"/>
            <rdf:Description rdf:about="http://www.w3.org/ns/ssn/deployedSystem"/>
        </owl:propertyChainAxiom>
        <rdfs:isDefinedBy rdf:resource="http://www.w3.org/ns/sosa/"/>
    </rdf:Description>
    


    <!-- http://www.w3.org/ns/sosa/isActedOnBy -->

    <rdf:Description rdf:about="http://www.w3.org/ns/sosa/isActedOnBy">
        <rdfs:domain rdf:resource="http://www.w3.org/ns/sosa/ActuatableProperty"/>
        <rdfs:range rdf:resource="http://www.w3.org/ns/sosa/Actuation"/>
        <rdfs:isDefinedBy rdf:resource="http://www.w3.org/ns/sosa/"/>
    </rdf:Description>
    


    <!-- http://www.w3.org/ns/sosa/isFeatureOfInterestOf -->

    <rdf:Description rdf:about="http://www.w3.org/ns/sosa/isFeatureOfInterestOf">
        <rdfs:domain rdf:resource="http://www.w3.org/ns/sosa/FeatureOfInterest"/>
        <rdfs:domain rdf:resource="http://www.w3.org/ns/sosa/Sample"/>
        <rdfs:range rdf:resource="http://www.w3.org/ns/sosa/Actuation"/>
        <rdfs:range rdf:resource="http://www.w3.org/ns/sosa/Observation"/>
        <rdfs:range rdf:resource="http://www.w3.org/ns/sosa/Sampling"/>
        <rdfs:isDefinedBy rdf:resource="http://www.w3.org/ns/sosa/"/>
    </rdf:Description>
    


    <!-- http://www.w3.org/ns/sosa/isHostedBy -->

    <rdf:Description rdf:about="http://www.w3.org/ns/sosa/isHostedBy">
        <rdfs:domain rdf:resource="http://www.w3.org/ns/sosa/Actuator"/>
        <rdfs:domain rdf:resource="http://www.w3.org/ns/sosa/Platform"/>
        <rdfs:domain rdf:resource="http://www.w3.org/ns/sosa/Sampler"/>
        <rdfs:domain rdf:resource="http://www.w3.org/ns/sosa/Sensor"/>
        <rdfs:range rdf:resource="http://www.w3.org/ns/sosa/Platform"/>
        <rdfs:isDefinedBy rdf:resource="http://www.w3.org/ns/sosa/"/>
    </rdf:Description>
    


    <!-- http://www.w3.org/ns/sosa/isObservedBy -->

    <rdf:Description rdf:about="http://www.w3.org/ns/sosa/isObservedBy">
        <rdfs:domain rdf:resource="http://www.w3.org/ns/sosa/ObservableProperty"/>
        <rdfs:range rdf:resource="http://www.w3.org/ns/sosa/Sensor"/>
        <rdfs:isDefinedBy rdf:resource="http://www.w3.org/ns/sosa/"/>
    </rdf:Description>
    


    <!-- http://www.w3.org/ns/sosa/isResultOf -->

    <rdf:Description rdf:about="http://www.w3.org/ns/sosa/isResultOf">
        <rdfs:domain rdf:resource="http://www.w3.org/ns/sosa/Result"/>
        <rdfs:domain rdf:resource="http://www.w3.org/ns/sosa/Sample"/>
        <rdfs:range rdf:resource="http://www.w3.org/ns/sosa/Actuation"/>
        <rdfs:range rdf:resource="http://www.w3.org/ns/sosa/Observation"/>
        <rdfs:range rdf:resource="http://www.w3.org/ns/sosa/Sampling"/>
        <rdfs:isDefinedBy rdf:resource="http://www.w3.org/ns/sosa/"/>
    </rdf:Description>
    


    <!-- http://www.w3.org/ns/sosa/isSampleOf -->

    <rdf:Description rdf:about="http://www.w3.org/ns/sosa/isSampleOf">
        <rdf:type rdf:resource="http://www.w3.org/2002/07/owl#FunctionalProperty"/>
        <rdfs:domain rdf:resource="http://www.w3.org/ns/sosa/Sample"/>
        <rdfs:range rdf:resource="http://www.w3.org/ns/sosa/FeatureOfInterest"/>
        <rdfs:isDefinedBy rdf:resource="http://www.w3.org/ns/sosa/"/>
    </rdf:Description>
    


    <!-- http://www.w3.org/ns/sosa/madeActuation -->

    <rdf:Description rdf:about="http://www.w3.org/ns/sosa/madeActuation">
        <rdfs:domain rdf:resource="http://www.w3.org/ns/sosa/Actuator"/>
        <rdfs:range rdf:resource="http://www.w3.org/ns/sosa/Actuation"/>
        <rdfs:isDefinedBy rdf:resource="http://www.w3.org/ns/sosa/"/>
    </rdf:Description>
    


    <!-- http://www.w3.org/ns/sosa/madeByActuator -->

    <rdf:Description rdf:about="http://www.w3.org/ns/sosa/madeByActuator">
        <rdfs:domain rdf:resource="http://www.w3.org/ns/sosa/Actuation"/>
        <rdfs:range rdf:resource="http://www.w3.org/ns/sosa/Actuator"/>
        <rdfs:isDefinedBy rdf:resource="http://www.w3.org/ns/sosa/"/>
    </rdf:Description>
    


    <!-- http://www.w3.org/ns/sosa/madeBySampler -->

    <rdf:Description rdf:about="http://www.w3.org/ns/sosa/madeBySampler">
        <rdfs:domain rdf:resource="http://www.w3.org/ns/sosa/Sampling"/>
        <rdfs:range rdf:resource="http://www.w3.org/ns/sosa/Sampler"/>
        <rdfs:isDefinedBy rdf:resource="http://www.w3.org/ns/sosa/"/>
    </rdf:Description>
    


    <!-- http://www.w3.org/ns/sosa/madeBySensor -->

    <rdf:Description rdf:about="http://www.w3.org/ns/sosa/madeBySensor">
        <rdfs:domain rdf:resource="http://www.w3.org/ns/sosa/Observation"/>
        <rdfs:range rdf:resource="http://www.w3.org/ns/sosa/Sensor"/>
        <rdfs:isDefinedBy rdf:resource="http://www.w3.org/ns/sosa/"/>
    </rdf:Description>
    


    <!-- http://www.w3.org/ns/sosa/madeObservation -->

    <rdf:Description rdf:about="http://www.w3.org/ns/sosa/madeObservation">
        <rdfs:domain rdf:resource="http://www.w3.org/ns/sosa/Sensor"/>
        <rdfs:range rdf:resource="http://www.w3.org/ns/sosa/Observation"/>
        <rdfs:isDefinedBy rdf:resource="http://www.w3.org/ns/sosa/"/>
    </rdf:Description>
    


    <!-- http://www.w3.org/ns/sosa/madeSampling -->

    <rdf:Description rdf:about="http://www.w3.org/ns/sosa/madeSampling">
        <rdfs:domain rdf:resource="http://www.w3.org/ns/sosa/Sampler"/>
        <rdfs:range rdf:resource="http://www.w3.org/ns/sosa/Sampling"/>
        <rdfs:isDefinedBy rdf:resource="http://www.w3.org/ns/sosa/"/>
    </rdf:Description>
    


    <!-- http://www.w3.org/ns/sosa/observedProperty -->

    <rdf:Description rdf:about="http://www.w3.org/ns/sosa/observedProperty">
        <rdfs:domain rdf:resource="http://www.w3.org/ns/sosa/Observation"/>
        <rdfs:range rdf:resource="http://www.w3.org/ns/sosa/ObservableProperty"/>
        <rdfs:isDefinedBy rdf:resource="http://www.w3.org/ns/sosa/"/>
    </rdf:Description>
    


    <!-- http://www.w3.org/ns/sosa/observes -->

    <rdf:Description rdf:about="http://www.w3.org/ns/sosa/observes">
        <rdfs:subPropertyOf rdf:resource="http://www.w3.org/ns/ssn/forProperty"/>
        <rdfs:domain rdf:resource="http://www.w3.org/ns/sosa/Sensor"/>
        <rdfs:range rdf:resource="http://www.w3.org/ns/sosa/ObservableProperty"/>
        <rdfs:isDefinedBy rdf:resource="http://www.w3.org/ns/sosa/"/>
    </rdf:Description>
    


    <!-- http://www.w3.org/ns/sosa/phenomenonTime -->

    <rdf:Description rdf:about="http://www.w3.org/ns/sosa/phenomenonTime">
        <rdfs:domain rdf:resource="http://www.w3.org/ns/sosa/Actuation"/>
        <rdfs:domain rdf:resource="http://www.w3.org/ns/sosa/Observation"/>
        <rdfs:domain rdf:resource="http://www.w3.org/ns/sosa/Sampling"/>
        <rdfs:range rdf:resource="http://www.w3.org/2006/time#TemporalEntity"/>
        <rdfs:isDefinedBy rdf:resource="http://www.w3.org/ns/sosa/"/>
    </rdf:Description>
    


    <!-- http://www.w3.org/ns/sosa/usedProcedure -->

    <rdf:Description rdf:about="http://www.w3.org/ns/sosa/usedProcedure">
        <rdfs:domain rdf:resource="http://www.w3.org/ns/sosa/Actuation"/>
        <rdfs:domain rdf:resource="http://www.w3.org/ns/sosa/Observation"/>
        <rdfs:domain rdf:resource="http://www.w3.org/ns/sosa/Sampling"/>
        <rdfs:range rdf:resource="http://www.w3.org/ns/sosa/Procedure"/>
        <owl:propertyChainAxiom rdf:parseType="Collection">
            <rdf:Description rdf:about="http://www.w3.org/ns/sosa/madeByActuator"/>
            <rdf:Description rdf:about="http://www.w3.org/ns/ssn/implements"/>
        </owl:propertyChainAxiom>
        <owl:propertyChainAxiom rdf:parseType="Collection">
            <rdf:Description rdf:about="http://www.w3.org/ns/sosa/madeBySampler"/>
            <rdf:Description rdf:about="http://www.w3.org/ns/ssn/implements"/>
        </owl:propertyChainAxiom>
        <owl:propertyChainAxiom rdf:parseType="Collection">
            <rdf:Description rdf:about="http://www.w3.org/ns/sosa/madeBySensor"/>
            <rdf:Description rdf:about="http://www.w3.org/ns/ssn/implements"/>
        </owl:propertyChainAxiom>
        <rdfs:isDefinedBy rdf:resource="http://www.w3.org/ns/sosa/"/>
    </rdf:Description>
    


    <!-- http://www.w3.org/ns/sosa/sampling/hasSampleRelationship -->

    <owl:ObjectProperty rdf:about="http://www.w3.org/ns/sosa/sampling/hasSampleRelationship">
        <rdfs:domain rdf:resource="http://www.w3.org/ns/sosa/Sample"/>
        <rdfs:range rdf:resource="http://www.w3.org/ns/sosa/sampling/SampleRelationship"/>
        <rdfs:comment>Links a sample to a Sample Relationship (which links to a related Sample).</rdfs:comment>
        <rdfs:isDefinedBy>http://www.w3.org/ns/sosa/sampling/</rdfs:isDefinedBy>
        <rdfs:label>has sample relationship</rdfs:label>
    </owl:ObjectProperty>
    


    <!-- http://www.w3.org/ns/sosa/sampling/natureOfRelationship -->

    <owl:ObjectProperty rdf:about="http://www.w3.org/ns/sosa/sampling/natureOfRelationship">
        <rdfs:domain rdf:resource="http://www.w3.org/ns/sosa/sampling/SampleRelationship"/>
        <rdfs:range rdf:resource="http://www.w3.org/ns/sosa/sampling/SampleRelationship"/>
        <rdfs:comment>Links a SampleRelationship to an indication of the nature of the relationship.</rdfs:comment>
        <rdfs:label>nature of relationship</rdfs:label>
    </owl:ObjectProperty>
    


    <!-- http://www.w3.org/ns/sosa/sampling/relatedSample -->

    <owl:ObjectProperty rdf:about="http://www.w3.org/ns/sosa/sampling/relatedSample">
        <rdfs:domain rdf:resource="http://www.w3.org/ns/sosa/sampling/SampleRelationship"/>
        <rdfs:range rdf:resource="http://www.w3.org/ns/sosa/Sample"/>
        <rdfs:comment>Links a SampleRelationship to the related Sample.</rdfs:comment>
        <rdfs:isDefinedBy>http://www.w3.org/ns/sosa/sampling/</rdfs:isDefinedBy>
        <rdfs:label>related sample</rdfs:label>
    </owl:ObjectProperty>
    


    <!-- http://www.w3.org/ns/ssn/deployedOnPlatform -->

    <owl:ObjectProperty rdf:about="http://www.w3.org/ns/ssn/deployedOnPlatform">
        <owl:inverseOf rdf:resource="http://www.w3.org/ns/ssn/inDeployment"/>
        <rdfs:domain rdf:resource="http://www.w3.org/ns/ssn/Deployment"/>
        <rdfs:range rdf:resource="http://www.w3.org/ns/sosa/Platform"/>
        <rdfs:comment xml:lang="en">Relation between a Deployment and the Platform on which the Systems are deployed.</rdfs:comment>
        <rdfs:isDefinedBy rdf:resource="http://www.w3.org/ns/ssn/"/>
        <rdfs:label xml:lang="en">deployed on platform</rdfs:label>
        <skos:definition xml:lang="en">Relation between a Deployment and the Platform on which the Systems are deployed.</skos:definition>
    </owl:ObjectProperty>
    


    <!-- http://www.w3.org/ns/ssn/deployedSystem -->

    <owl:ObjectProperty rdf:about="http://www.w3.org/ns/ssn/deployedSystem">
        <owl:inverseOf rdf:resource="http://www.w3.org/ns/ssn/hasDeployment"/>
        <rdfs:domain rdf:resource="http://www.w3.org/ns/ssn/Deployment"/>
        <rdfs:range rdf:resource="http://www.w3.org/ns/ssn/System"/>
        <rdfs:comment xml:lang="en">Relation between a Deployment and a deployed System.</rdfs:comment>
        <rdfs:isDefinedBy rdf:resource="http://www.w3.org/ns/ssn/"/>
        <rdfs:label xml:lang="en">deployed system</rdfs:label>
        <skos:definition xml:lang="en">Relation between a Deployment and a deployed System.</skos:definition>
    </owl:ObjectProperty>
    


    <!-- http://www.w3.org/ns/ssn/detects -->

    <owl:ObjectProperty rdf:about="http://www.w3.org/ns/ssn/detects">
        <rdfs:domain rdf:resource="http://www.w3.org/ns/sosa/Sensor"/>
        <rdfs:range rdf:resource="http://www.w3.org/ns/ssn/Stimulus"/>
        <rdfs:comment xml:lang="en">A relation from a Sensor to the Stimulus that the Sensor detects. The Stimulus itself will be serving as a proxy for some ObservableProperty.</rdfs:comment>
        <rdfs:isDefinedBy rdf:resource="http://www.w3.org/ns/ssn/"/>
        <rdfs:label xml:lang="en">detects</rdfs:label>
        <skos:definition xml:lang="en">A relation from a Sensor to the Stimulus that the Sensor detects. The Stimulus itself will be serving as a proxy for some ObservableProperty.</skos:definition>
    </owl:ObjectProperty>
    


    <!-- http://www.w3.org/ns/ssn/forProperty -->

    <owl:ObjectProperty rdf:about="http://www.w3.org/ns/ssn/forProperty">
        <rdfs:range rdf:resource="http://www.w3.org/ns/ssn/Property"/>
        <rdfs:comment xml:lang="en">A relation between some aspect of an entity and a Property.</rdfs:comment>
        <rdfs:isDefinedBy rdf:resource="http://www.w3.org/ns/ssn/"/>
        <rdfs:label xml:lang="en">for property</rdfs:label>
        <skos:definition xml:lang="en">A relation between some aspect of an entity and a Property.</skos:definition>
        <skos:example xml:lang="en">For example, from a Sensor to the properties it can observe; from an Actuator to the properties it can act on; from a Deployment to the properties it was installed to observe or act on; from a SystemCapability to the Property the capability is described for.</skos:example>
    </owl:ObjectProperty>
    


    <!-- http://www.w3.org/ns/ssn/hasDeployment -->

    <owl:ObjectProperty rdf:about="http://www.w3.org/ns/ssn/hasDeployment">
        <rdfs:domain rdf:resource="http://www.w3.org/ns/ssn/System"/>
        <rdfs:range rdf:resource="http://www.w3.org/ns/ssn/Deployment"/>
        <rdfs:comment xml:lang="en">Relation between a System and a Deployment, recording that the System is deployed in that Deployment.</rdfs:comment>
        <rdfs:isDefinedBy rdf:resource="http://www.w3.org/ns/ssn/"/>
        <rdfs:label xml:lang="en">has deployment</rdfs:label>
        <skos:definition xml:lang="en">Relation between a System and a Deployment, recording that the System is deployed in that Deployment.</skos:definition>
    </owl:ObjectProperty>
    


    <!-- http://www.w3.org/ns/ssn/hasInput -->

    <owl:ObjectProperty rdf:about="http://www.w3.org/ns/ssn/hasInput">
        <rdfs:domain rdf:resource="http://www.w3.org/ns/sosa/Procedure"/>
        <rdfs:range rdf:resource="http://www.w3.org/ns/ssn/Input"/>
        <rdfs:comment xml:lang="en">Relation between a Procedure and an Input to it.</rdfs:comment>
        <rdfs:isDefinedBy rdf:resource="http://www.w3.org/ns/ssn/"/>
        <rdfs:label xml:lang="en">has input</rdfs:label>
        <skos:definition xml:lang="en">Relation between a Procedure and an Input to it.</skos:definition>
    </owl:ObjectProperty>
    


    <!-- http://www.w3.org/ns/ssn/hasOutput -->

    <owl:ObjectProperty rdf:about="http://www.w3.org/ns/ssn/hasOutput">
        <rdfs:domain rdf:resource="http://www.w3.org/ns/sosa/Procedure"/>
        <rdfs:range rdf:resource="http://www.w3.org/ns/ssn/Output"/>
        <rdfs:comment xml:lang="en">Relation between a Procedure and an Output of it.</rdfs:comment>
        <rdfs:isDefinedBy rdf:resource="http://www.w3.org/ns/ssn/"/>
        <rdfs:label xml:lang="en">has output</rdfs:label>
        <skos:definition xml:lang="en">Relation between a Procedure and an Output of it.</skos:definition>
    </owl:ObjectProperty>
    


    <!-- http://www.w3.org/ns/ssn/hasProperty -->

    <owl:ObjectProperty rdf:about="http://www.w3.org/ns/ssn/hasProperty">
        <owl:inverseOf rdf:resource="http://www.w3.org/ns/ssn/isPropertyOf"/>
        <rdfs:range rdf:resource="http://www.w3.org/ns/ssn/Property"/>
        <rdfs:comment xml:lang="en">Relation between an entity and a Property of that entity.</rdfs:comment>
        <rdfs:isDefinedBy rdf:resource="http://www.w3.org/ns/ssn/"/>
        <rdfs:label xml:lang="en">has property</rdfs:label>
        <skos:definition xml:lang="en">Relation between an entity and a Property of that entity.</skos:definition>
    </owl:ObjectProperty>
    


    <!-- http://www.w3.org/ns/ssn/hasSubSystem -->

    <owl:ObjectProperty rdf:about="http://www.w3.org/ns/ssn/hasSubSystem">
        <rdfs:domain rdf:resource="http://www.w3.org/ns/ssn/System"/>
        <rdfs:range rdf:resource="http://www.w3.org/ns/ssn/System"/>
        <rdfs:comment xml:lang="en">Relation between a System and its component parts.</rdfs:comment>
        <rdfs:isDefinedBy rdf:resource="http://www.w3.org/ns/ssn/"/>
        <rdfs:label xml:lang="en">has subsystem</rdfs:label>
        <skos:definition xml:lang="en">Relation between a System and its component parts.</skos:definition>
    </owl:ObjectProperty>
    


    <!-- http://www.w3.org/ns/ssn/implementedBy -->

    <owl:ObjectProperty rdf:about="http://www.w3.org/ns/ssn/implementedBy">
        <owl:inverseOf rdf:resource="http://www.w3.org/ns/ssn/implements"/>
        <rdfs:domain rdf:resource="http://www.w3.org/ns/sosa/Procedure"/>
        <rdfs:comment xml:lang="en">Relation between a Procedure (an algorithm, procedure or method) and an entity that implements that Procedure in some executable way.</rdfs:comment>
        <rdfs:isDefinedBy rdf:resource="http://www.w3.org/ns/ssn/"/>
        <rdfs:label xml:lang="en">implemented by</rdfs:label>
        <skos:definition xml:lang="en">Relation between a Procedure (an algorithm, procedure or method) and an entity that implements that Procedure in some executable way.</skos:definition>
        <skos:example xml:lang="en">For example, the relationship between a scientific measuring Procedure and a sensor that senses via that Procedure.</skos:example>
    </owl:ObjectProperty>
    


    <!-- http://www.w3.org/ns/ssn/implements -->

    <owl:ObjectProperty rdf:about="http://www.w3.org/ns/ssn/implements">
        <rdfs:range rdf:resource="http://www.w3.org/ns/sosa/Procedure"/>
        <rdfs:comment xml:lang="en">Relation between an entity that implements a Procedure in some executable way and the Procedure (an algorithm, procedure or method).</rdfs:comment>
        <rdfs:isDefinedBy rdf:resource="http://www.w3.org/ns/ssn/"/>
        <rdfs:label xml:lang="en">implements</rdfs:label>
        <skos:definition xml:lang="en">Relation between an entity that implements a Procedure in some executable way and the Procedure (an algorithm, procedure or method).</skos:definition>
        <skos:example xml:lang="en">For example, the relationship between a sensor and the scientific measuring Procedure via which it senses.</skos:example>
    </owl:ObjectProperty>
    


    <!-- http://www.w3.org/ns/ssn/inDeployment -->

    <owl:ObjectProperty rdf:about="http://www.w3.org/ns/ssn/inDeployment">
        <rdfs:domain rdf:resource="http://www.w3.org/ns/sosa/Platform"/>
        <rdfs:range rdf:resource="http://www.w3.org/ns/ssn/Deployment"/>
        <rdfs:comment xml:lang="en">Relation between a Platform and a Deployment, meaning that the deployedSystems of the Deployment are hosted on the Platform.</rdfs:comment>
        <rdfs:isDefinedBy rdf:resource="http://www.w3.org/ns/ssn/"/>
        <rdfs:label xml:lang="en">in deployment</rdfs:label>
        <skos:definition xml:lang="en">Relation between a Platform and a Deployment, meaning that the deployedSystems of the Deployment are hosted on the Platform.</skos:definition>
        <skos:example xml:lang="en">For example, a relation between a buoy and a deployment of several Sensors.</skos:example>
    </owl:ObjectProperty>
    


    <!-- http://www.w3.org/ns/ssn/isPropertyOf -->

    <owl:ObjectProperty rdf:about="http://www.w3.org/ns/ssn/isPropertyOf">
        <rdfs:domain rdf:resource="http://www.w3.org/ns/ssn/Property"/>
        <rdfs:comment xml:lang="en">Relation between a Property and the entity it belongs to.</rdfs:comment>
        <rdfs:isDefinedBy rdf:resource="http://www.w3.org/ns/ssn/"/>
        <rdfs:label xml:lang="en">is property of</rdfs:label>
        <skos:definition xml:lang="en">Relation between a Property and the entity it belongs to.</skos:definition>
    </owl:ObjectProperty>
    


    <!-- http://www.w3.org/ns/ssn/isProxyFor -->

    <owl:ObjectProperty rdf:about="http://www.w3.org/ns/ssn/isProxyFor">
        <rdfs:domain rdf:resource="http://www.w3.org/ns/ssn/Stimulus"/>
        <rdfs:range rdf:resource="http://www.w3.org/ns/ssn/Property"/>
        <rdfs:comment xml:lang="en">A relation from a Stimulus to the Property that the Stimulus is serving as a proxy for.</rdfs:comment>
        <rdfs:isDefinedBy rdf:resource="http://www.w3.org/ns/ssn/"/>
        <rdfs:label xml:lang="en">is proxy for</rdfs:label>
        <skos:definition xml:lang="en">A relation from a Stimulus to the Property that the Stimulus is serving as a proxy for.</skos:definition>
        <skos:example xml:lang="en">For example, the expansion of quicksilver is a stimulus that serves as a proxy for some temperature property. An increase or decrease in the velocity of spinning cups on a wind sensor is serving as a proxy for the wind speed.</skos:example>
    </owl:ObjectProperty>
    


    <!-- http://www.w3.org/ns/ssn/oversamplingUsed -->

    <owl:ObjectProperty rdf:about="http://www.w3.org/ns/ssn/oversamplingUsed">
        <rdfs:domain rdf:resource="http://www.w3.org/ns/sosa/Observation"/>
        <rdfs:range rdf:resource="http://www.w3.org/ns/ssn/OversamplingRate"/>
        <rdfs:comment>Link to the oversampling rate.</rdfs:comment>
        <rdfs:label>oversampling used</rdfs:label>
    </owl:ObjectProperty>
    


    <!-- http://www.w3.org/ns/ssn/wasOriginatedBy -->

    <owl:ObjectProperty rdf:about="http://www.w3.org/ns/ssn/wasOriginatedBy">
        <rdf:type rdf:resource="http://www.w3.org/2002/07/owl#FunctionalProperty"/>
        <rdfs:domain rdf:resource="http://www.w3.org/ns/sosa/Observation"/>
        <rdfs:range rdf:resource="http://www.w3.org/ns/ssn/Stimulus"/>
        <rdfs:comment xml:lang="en">Relation between an Observation and the Stimulus that originated it.</rdfs:comment>
        <rdfs:isDefinedBy rdf:resource="http://www.w3.org/ns/ssn/"/>
        <rdfs:label xml:lang="en">was originated by</rdfs:label>
        <skos:definition xml:lang="en">Relation between an Observation and the Stimulus that originated it.</skos:definition>
    </owl:ObjectProperty>
    


    <!-- http://www.w3.org/ns/ssn/systems/hasOperatingProperty -->

    <owl:ObjectProperty rdf:about="http://www.w3.org/ns/ssn/systems/hasOperatingProperty">
        <rdfs:subPropertyOf rdf:resource="http://www.w3.org/ns/ssn/hasProperty"/>
        <rdfs:domain rdf:resource="http://www.w3.org/ns/ssn/systems/OperatingRange"/>
        <rdfs:range rdf:resource="http://www.w3.org/ns/ssn/systems/OperatingProperty"/>
        <rdfs:comment>Relation from an OperatingRange of a System to an OperatingProperty describing the operating range of the System.</rdfs:comment>
        <rdfs:isDefinedBy rdf:resource="http://www.w3.org/ns/ssn/systems/"/>
        <rdfs:label>has operating property</rdfs:label>
    </owl:ObjectProperty>
    


    <!-- http://www.w3.org/ns/ssn/systems/hasOperatingRange -->

    <owl:ObjectProperty rdf:about="http://www.w3.org/ns/ssn/systems/hasOperatingRange">
        <rdfs:subPropertyOf rdf:resource="http://www.w3.org/ns/ssn/hasProperty"/>
        <rdfs:domain rdf:resource="http://www.w3.org/ns/ssn/System"/>
        <rdfs:range rdf:resource="http://www.w3.org/ns/ssn/systems/OperatingRange"/>
        <rdfs:comment>Relation from a System to an OperatingRange describing the normal operating environment of the System.</rdfs:comment>
        <rdfs:isDefinedBy rdf:resource="http://www.w3.org/ns/ssn/systems/"/>
        <rdfs:label>has operating range</rdfs:label>
    </owl:ObjectProperty>
    


    <!-- http://www.w3.org/ns/ssn/systems/hasSurvivalProperty -->

    <owl:ObjectProperty rdf:about="http://www.w3.org/ns/ssn/systems/hasSurvivalProperty">
        <rdfs:subPropertyOf rdf:resource="http://www.w3.org/ns/ssn/hasProperty"/>
        <rdfs:domain rdf:resource="http://www.w3.org/ns/ssn/systems/SurvivalRange"/>
        <rdfs:range rdf:resource="http://www.w3.org/ns/ssn/systems/SurvivalProperty"/>
        <rdfs:comment>Relation from a SurvivalRange of a System to a SurvivalProperty describing the survival range of the System.</rdfs:comment>
        <rdfs:isDefinedBy rdf:resource="http://www.w3.org/ns/ssn/systems/"/>
        <rdfs:label>has survival property</rdfs:label>
    </owl:ObjectProperty>
    


    <!-- http://www.w3.org/ns/ssn/systems/hasSurvivalRange -->

    <owl:ObjectProperty rdf:about="http://www.w3.org/ns/ssn/systems/hasSurvivalRange">
        <rdfs:subPropertyOf rdf:resource="http://www.w3.org/ns/ssn/hasProperty"/>
        <rdfs:domain rdf:resource="http://www.w3.org/ns/ssn/System"/>
        <rdfs:range rdf:resource="http://www.w3.org/ns/ssn/systems/SurvivalRange"/>
        <rdfs:comment>Relation from a System to SurvivalRange.</rdfs:comment>
        <rdfs:isDefinedBy rdf:resource="http://www.w3.org/ns/ssn/systems/"/>
        <rdfs:label>has survival range</rdfs:label>
    </owl:ObjectProperty>
    


    <!-- http://www.w3.org/ns/ssn/systems/hasSystemCapability -->

    <owl:ObjectProperty rdf:about="http://www.w3.org/ns/ssn/systems/hasSystemCapability">
        <rdfs:subPropertyOf rdf:resource="http://www.w3.org/ns/ssn/hasProperty"/>
        <rdfs:domain rdf:resource="http://www.w3.org/ns/ssn/System"/>
        <rdfs:range rdf:resource="http://www.w3.org/ns/ssn/systems/SystemCapability"/>
        <rdfs:comment>Relation from a System to a SystemCapability describing the capabilities of the System under certain Conditions.</rdfs:comment>
        <rdfs:isDefinedBy rdf:resource="http://www.w3.org/ns/ssn/systems/"/>
        <rdfs:label>has system capability</rdfs:label>
    </owl:ObjectProperty>
    


    <!-- http://www.w3.org/ns/ssn/systems/hasSystemProperty -->

    <owl:ObjectProperty rdf:about="http://www.w3.org/ns/ssn/systems/hasSystemProperty">
        <rdfs:subPropertyOf rdf:resource="http://www.w3.org/ns/ssn/hasProperty"/>
        <rdfs:domain rdf:resource="http://www.w3.org/ns/ssn/systems/SystemCapability"/>
        <rdfs:range rdf:resource="http://www.w3.org/ns/ssn/systems/SystemProperty"/>
        <rdfs:comment>Relation from a SystemCapability of a System to a SystemProperty describing the capabilities of the System.</rdfs:comment>
        <rdfs:isDefinedBy rdf:resource="http://www.w3.org/ns/ssn/systems/"/>
        <rdfs:label>has system property</rdfs:label>
    </owl:ObjectProperty>
    


    <!-- http://www.w3.org/ns/ssn/systems/inCondition -->

    <owl:ObjectProperty rdf:about="http://www.w3.org/ns/ssn/systems/inCondition">
        <rdfs:domain rdf:resource="http://www.w3.org/ns/ssn/systems/OperatingRange"/>
        <rdfs:domain rdf:resource="http://www.w3.org/ns/ssn/systems/SurvivalRange"/>
        <rdfs:domain rdf:resource="http://www.w3.org/ns/ssn/systems/SystemCapability"/>
        <rdfs:range rdf:resource="http://www.w3.org/ns/ssn/Condition"/>
        <rdfs:comment>Describes the prevailing environmental Conditions for SystemCapabilities, OperatingRanges and SurvivalRanges.</rdfs:comment>
        <rdfs:isDefinedBy rdf:resource="http://www.w3.org/ns/ssn/systems/"/>
        <rdfs:label>in condition</rdfs:label>
        <skos:example>Used for example to say that a Sensor has a particular accuracy in particular Conditions.</skos:example>
    </owl:ObjectProperty>
    


    <!-- http://www.w3.org/ns/ssn/systems/qualityOfObservation -->

    <owl:ObjectProperty rdf:about="http://www.w3.org/ns/ssn/systems/qualityOfObservation">
        <rdfs:subPropertyOf rdf:resource="http://www.w3.org/ns/ssn/hasProperty"/>
        <rdfs:domain rdf:resource="http://www.w3.org/ns/sosa/Observation"/>
        <rdfs:range rdf:resource="http://www.w3.org/ns/sosa/Result"/>
        <rdfs:comment>Relation linking an Observation to the adjudged quality of the Result. This is complementary to the SystemCapability information recorded for the Sensor that made the Observation.</rdfs:comment>
        <rdfs:isDefinedBy rdf:resource="http://www.w3.org/ns/ssn/systems/"/>
        <rdfs:label>quality of observation</rdfs:label>
    </owl:ObjectProperty>
    


    <!-- 
    ///////////////////////////////////////////////////////////////////////////////////////
    //
    // Data properties
    //
    ///////////////////////////////////////////////////////////////////////////////////////
     -->

    


    <!-- http://www.w3.org/ns/sosa/resultTime -->

    <rdf:Description rdf:about="http://www.w3.org/ns/sosa/resultTime">
        <rdfs:isDefinedBy rdf:resource="http://www.w3.org/ns/sosa/"/>
    </rdf:Description>
    


    <!-- 
    ///////////////////////////////////////////////////////////////////////////////////////
    //
    // Classes
    //
    ///////////////////////////////////////////////////////////////////////////////////////
     -->

    


    <!-- http://purl.org/vocommons/voaf#Vocabulary -->

    <owl:Class rdf:about="http://purl.org/vocommons/voaf#Vocabulary"/>
    


    <!-- http://www.w3.org/2006/time#TemporalEntity -->

    <owl:Class rdf:about="http://www.w3.org/2006/time#TemporalEntity">
        <rdfs:comment>A temporal interval or instant.</rdfs:comment>
        <rdfs:isDefinedBy>http://www.w3.org/TR/owl-time/#time:TemporalEntity</rdfs:isDefinedBy>
        <rdfs:label>Temporal entity</rdfs:label>
    </owl:Class>
    


    <!-- http://www.w3.org/TR/vocab-ssn-ext/ObservationCollection -->

    <owl:Class rdf:about="http://www.w3.org/TR/vocab-ssn-ext/ObservationCollection">
        <rdfs:subClassOf>
            <owl:Restriction>
                <owl:onProperty rdf:resource="http://www.w3.org/TR/vocab-ssn-ext/hasMember"/>
                <owl:minCardinality rdf:datatype="http://www.w3.org/2001/XMLSchema#nonNegativeInteger">1</owl:minCardinality>
            </owl:Restriction>
        </rdfs:subClassOf>
        <rdfs:subClassOf>
            <owl:Restriction>
                <owl:onProperty rdf:resource="http://www.w3.org/TR/vocab-ssn-ext/hasUltimateFeatureOfInterest"/>
                <owl:maxCardinality rdf:datatype="http://www.w3.org/2001/XMLSchema#nonNegativeInteger">1</owl:maxCardinality>
            </owl:Restriction>
        </rdfs:subClassOf>
        <rdfs:subClassOf>
            <owl:Restriction>
                <owl:onProperty rdf:resource="http://www.w3.org/ns/sosa/hasFeatureOfInterest"/>
                <owl:maxCardinality rdf:datatype="http://www.w3.org/2001/XMLSchema#nonNegativeInteger">1</owl:maxCardinality>
            </owl:Restriction>
        </rdfs:subClassOf>
        <rdfs:subClassOf>
            <owl:Restriction>
                <owl:onProperty rdf:resource="http://www.w3.org/ns/sosa/madeBySensor"/>
                <owl:maxCardinality rdf:datatype="http://www.w3.org/2001/XMLSchema#nonNegativeInteger">1</owl:maxCardinality>
            </owl:Restriction>
        </rdfs:subClassOf>
        <rdfs:subClassOf>
            <owl:Restriction>
                <owl:onProperty rdf:resource="http://www.w3.org/ns/sosa/observedProperty"/>
                <owl:maxCardinality rdf:datatype="http://www.w3.org/2001/XMLSchema#nonNegativeInteger">1</owl:maxCardinality>
            </owl:Restriction>
        </rdfs:subClassOf>
        <rdfs:subClassOf>
            <owl:Restriction>
                <owl:onProperty rdf:resource="http://www.w3.org/ns/sosa/phenomenonTime"/>
                <owl:maxCardinality rdf:datatype="http://www.w3.org/2001/XMLSchema#nonNegativeInteger">1</owl:maxCardinality>
            </owl:Restriction>
        </rdfs:subClassOf>
        <rdfs:subClassOf>
            <owl:Restriction>
                <owl:onProperty rdf:resource="http://www.w3.org/ns/sosa/resultTime"/>
                <owl:maxQualifiedCardinality rdf:datatype="http://www.w3.org/2001/XMLSchema#nonNegativeInteger">1</owl:maxQualifiedCardinality>
                <owl:onDataRange rdf:resource="http://www.w3.org/2002/07/owl#rational"/>
            </owl:Restriction>
        </rdfs:subClassOf>
        <rdfs:comment>An Observation Collection has at least one member, and may have one of any of the other seven properties mentioned in restrictions.</rdfs:comment>
        <rdfs:isDefinedBy>http://www.w3.org/ns/ssn/ext/ObservationCollection</rdfs:isDefinedBy>
    </owl:Class>
    


    <!-- http://www.w3.org/ns/sosa/ActuatableProperty -->

    <rdf:Description rdf:about="http://www.w3.org/ns/sosa/ActuatableProperty">
        <rdfs:subClassOf rdf:resource="http://www.w3.org/ns/ssn/Property"/>
        <rdfs:subClassOf>
            <owl:Restriction>
                <owl:onProperty rdf:resource="http://www.w3.org/ns/sosa/isActedOnBy"/>
                <owl:allValuesFrom rdf:resource="http://www.w3.org/ns/sosa/Actuation"/>
            </owl:Restriction>
        </rdfs:subClassOf>
        <rdfs:isDefinedBy rdf:resource="http://www.w3.org/ns/sosa/"/>
    </rdf:Description>
    


    <!-- http://www.w3.org/ns/sosa/Actuation -->

    <owl:Class rdf:about="http://www.w3.org/ns/sosa/Actuation">
        <rdfs:subClassOf>
            <owl:Restriction>
                <owl:onProperty rdf:resource="http://www.w3.org/ns/sosa/actsOnProperty"/>
                <owl:allValuesFrom rdf:resource="http://www.w3.org/ns/sosa/ActuatableProperty"/>
            </owl:Restriction>
        </rdfs:subClassOf>
        <rdfs:subClassOf>
            <owl:Restriction>
                <owl:onProperty rdf:resource="http://www.w3.org/ns/sosa/hasFeatureOfInterest"/>
                <owl:allValuesFrom rdf:resource="http://www.w3.org/ns/sosa/FeatureOfInterest"/>
            </owl:Restriction>
        </rdfs:subClassOf>
        <rdfs:subClassOf>
            <owl:Restriction>
                <owl:onProperty rdf:resource="http://www.w3.org/ns/sosa/hasResult"/>
                <owl:allValuesFrom rdf:resource="http://www.w3.org/ns/sosa/Result"/>
            </owl:Restriction>
        </rdfs:subClassOf>
        <rdfs:subClassOf>
            <owl:Restriction>
                <owl:onProperty rdf:resource="http://www.w3.org/ns/sosa/madeByActuator"/>
                <owl:allValuesFrom rdf:resource="http://www.w3.org/ns/sosa/Actuator"/>
            </owl:Restriction>
        </rdfs:subClassOf>
        <rdfs:subClassOf>
            <owl:Restriction>
                <owl:onProperty rdf:resource="http://www.w3.org/ns/sosa/usedProcedure"/>
                <owl:allValuesFrom rdf:resource="http://www.w3.org/ns/sosa/Procedure"/>
            </owl:Restriction>
        </rdfs:subClassOf>
        <rdfs:subClassOf>
            <owl:Restriction>
                <owl:onProperty rdf:resource="http://www.w3.org/ns/sosa/actsOnProperty"/>
                <owl:minCardinality rdf:datatype="http://www.w3.org/2001/XMLSchema#nonNegativeInteger">1</owl:minCardinality>
            </owl:Restriction>
        </rdfs:subClassOf>
        <rdfs:subClassOf>
            <owl:Restriction>
                <owl:onProperty rdf:resource="http://www.w3.org/ns/sosa/hasResult"/>
                <owl:minCardinality rdf:datatype="http://www.w3.org/2001/XMLSchema#nonNegativeInteger">1</owl:minCardinality>
            </owl:Restriction>
        </rdfs:subClassOf>
        <rdfs:subClassOf>
            <owl:Restriction>
                <owl:onProperty rdf:resource="http://www.w3.org/ns/sosa/hasFeatureOfInterest"/>
                <owl:cardinality rdf:datatype="http://www.w3.org/2001/XMLSchema#nonNegativeInteger">1</owl:cardinality>
            </owl:Restriction>
        </rdfs:subClassOf>
        <rdfs:subClassOf>
            <owl:Restriction>
                <owl:onProperty rdf:resource="http://www.w3.org/ns/sosa/madeByActuator"/>
                <owl:cardinality rdf:datatype="http://www.w3.org/2001/XMLSchema#nonNegativeInteger">1</owl:cardinality>
            </owl:Restriction>
        </rdfs:subClassOf>
        <rdfs:subClassOf>
            <owl:Restriction>
                <owl:onProperty rdf:resource="http://www.w3.org/ns/sosa/resultTime"/>
                <owl:cardinality rdf:datatype="http://www.w3.org/2001/XMLSchema#nonNegativeInteger">1</owl:cardinality>
            </owl:Restriction>
        </rdfs:subClassOf>
        <rdfs:isDefinedBy rdf:resource="http://www.w3.org/ns/sosa/"/>
    </owl:Class>
    


    <!-- http://www.w3.org/ns/sosa/Actuator -->

    <rdf:Description rdf:about="http://www.w3.org/ns/sosa/Actuator">
        <rdfs:subClassOf rdf:resource="http://www.w3.org/ns/ssn/System"/>
        <rdfs:subClassOf>
            <owl:Restriction>
                <owl:onProperty rdf:resource="http://www.w3.org/ns/sosa/madeActuation"/>
                <owl:allValuesFrom rdf:resource="http://www.w3.org/ns/sosa/Actuation"/>
            </owl:Restriction>
        </rdfs:subClassOf>
        <rdfs:subClassOf>
            <owl:Restriction>
                <owl:onProperty rdf:resource="http://www.w3.org/ns/ssn/forProperty"/>
                <owl:allValuesFrom rdf:resource="http://www.w3.org/ns/sosa/ActuatableProperty"/>
            </owl:Restriction>
        </rdfs:subClassOf>
        <rdfs:subClassOf>
            <owl:Restriction>
                <owl:onProperty rdf:resource="http://www.w3.org/ns/ssn/implements"/>
                <owl:minCardinality rdf:datatype="http://www.w3.org/2001/XMLSchema#nonNegativeInteger">1</owl:minCardinality>
            </owl:Restriction>
        </rdfs:subClassOf>
        <rdfs:isDefinedBy rdf:resource="http://www.w3.org/ns/sosa/"/>
    </rdf:Description>
    


    <!-- http://www.w3.org/ns/sosa/FeatureOfInterest -->

    <rdf:Description rdf:about="http://www.w3.org/ns/sosa/FeatureOfInterest">
        <rdfs:subClassOf>
            <owl:Restriction>
                <owl:onProperty rdf:resource="http://www.w3.org/ns/sosa/hasSample"/>
                <owl:allValuesFrom rdf:resource="http://www.w3.org/ns/sosa/Sample"/>
            </owl:Restriction>
        </rdfs:subClassOf>
        <rdfs:subClassOf>
            <owl:Restriction>
                <owl:onProperty rdf:resource="http://www.w3.org/ns/ssn/hasProperty"/>
                <owl:allValuesFrom rdf:resource="http://www.w3.org/ns/ssn/Property"/>
            </owl:Restriction>
        </rdfs:subClassOf>
        <rdfs:subClassOf>
            <owl:Restriction>
                <owl:onProperty rdf:resource="http://www.w3.org/ns/ssn/hasProperty"/>
                <owl:minCardinality rdf:datatype="http://www.w3.org/2001/XMLSchema#nonNegativeInteger">1</owl:minCardinality>
            </owl:Restriction>
        </rdfs:subClassOf>
        <rdfs:isDefinedBy rdf:resource="http://www.w3.org/ns/sosa/"/>
    </rdf:Description>
    


    <!-- http://www.w3.org/ns/sosa/ObservableProperty -->

    <rdf:Description rdf:about="http://www.w3.org/ns/sosa/ObservableProperty">
        <rdfs:subClassOf rdf:resource="http://www.w3.org/ns/ssn/Property"/>
        <rdfs:subClassOf>
            <owl:Restriction>
                <owl:onProperty rdf:resource="http://www.w3.org/ns/sosa/isObservedBy"/>
                <owl:allValuesFrom rdf:resource="http://www.w3.org/ns/sosa/Sensor"/>
            </owl:Restriction>
        </rdfs:subClassOf>
        <rdfs:subClassOf>
            <owl:Restriction>
                <owl:onProperty>
                    <rdf:Description>
                        <owl:inverseOf rdf:resource="http://www.w3.org/ns/sosa/observedProperty"/>
                    </rdf:Description>
                </owl:onProperty>
                <owl:allValuesFrom rdf:resource="http://www.w3.org/ns/sosa/Observation"/>
            </owl:Restriction>
        </rdfs:subClassOf>
        <rdfs:subClassOf>
            <owl:Restriction>
                <owl:onProperty>
                    <rdf:Description>
                        <owl:inverseOf rdf:resource="http://www.w3.org/ns/ssn/isProxyFor"/>
                    </rdf:Description>
                </owl:onProperty>
                <owl:allValuesFrom rdf:resource="http://www.w3.org/ns/ssn/Stimulus"/>
            </owl:Restriction>
        </rdfs:subClassOf>
        <rdfs:isDefinedBy rdf:resource="http://www.w3.org/ns/sosa/"/>
    </rdf:Description>
    


    <!-- http://www.w3.org/ns/sosa/Observation -->

    <owl:Class rdf:about="http://www.w3.org/ns/sosa/Observation">
        <rdfs:subClassOf>
            <owl:Restriction>
                <owl:onProperty rdf:resource="http://www.w3.org/ns/sosa/hasFeatureOfInterest"/>
                <owl:allValuesFrom rdf:resource="http://www.w3.org/ns/sosa/FeatureOfInterest"/>
            </owl:Restriction>
        </rdfs:subClassOf>
        <rdfs:subClassOf>
            <owl:Restriction>
                <owl:onProperty rdf:resource="http://www.w3.org/ns/sosa/hasResult"/>
                <owl:allValuesFrom rdf:resource="http://www.w3.org/ns/sosa/Result"/>
            </owl:Restriction>
        </rdfs:subClassOf>
        <rdfs:subClassOf>
            <owl:Restriction>
                <owl:onProperty rdf:resource="http://www.w3.org/ns/sosa/madeBySensor"/>
                <owl:allValuesFrom rdf:resource="http://www.w3.org/ns/sosa/Sensor"/>
            </owl:Restriction>
        </rdfs:subClassOf>
        <rdfs:subClassOf>
            <owl:Restriction>
                <owl:onProperty rdf:resource="http://www.w3.org/ns/sosa/observedProperty"/>
                <owl:allValuesFrom rdf:resource="http://www.w3.org/ns/sosa/ObservableProperty"/>
            </owl:Restriction>
        </rdfs:subClassOf>
        <rdfs:subClassOf>
            <owl:Restriction>
                <owl:onProperty rdf:resource="http://www.w3.org/ns/sosa/usedProcedure"/>
                <owl:allValuesFrom rdf:resource="http://www.w3.org/ns/sosa/Procedure"/>
            </owl:Restriction>
        </rdfs:subClassOf>
        <rdfs:subClassOf>
            <owl:Restriction>
                <owl:onProperty rdf:resource="http://www.w3.org/ns/ssn/wasOriginatedBy"/>
                <owl:allValuesFrom rdf:resource="http://www.w3.org/ns/ssn/Stimulus"/>
            </owl:Restriction>
        </rdfs:subClassOf>
        <rdfs:subClassOf>
            <owl:Restriction>
                <owl:onProperty rdf:resource="http://www.w3.org/ns/sosa/hasResult"/>
                <owl:minCardinality rdf:datatype="http://www.w3.org/2001/XMLSchema#nonNegativeInteger">1</owl:minCardinality>
            </owl:Restriction>
        </rdfs:subClassOf>
        <rdfs:subClassOf>
            <owl:Restriction>
                <owl:onProperty rdf:resource="http://www.w3.org/ns/sosa/hasFeatureOfInterest"/>
                <owl:cardinality rdf:datatype="http://www.w3.org/2001/XMLSchema#nonNegativeInteger">1</owl:cardinality>
            </owl:Restriction>
        </rdfs:subClassOf>
        <rdfs:subClassOf>
            <owl:Restriction>
                <owl:onProperty rdf:resource="http://www.w3.org/ns/sosa/madeBySensor"/>
                <owl:cardinality rdf:datatype="http://www.w3.org/2001/XMLSchema#nonNegativeInteger">1</owl:cardinality>
            </owl:Restriction>
        </rdfs:subClassOf>
        <rdfs:subClassOf>
            <owl:Restriction>
                <owl:onProperty rdf:resource="http://www.w3.org/ns/sosa/observedProperty"/>
                <owl:cardinality rdf:datatype="http://www.w3.org/2001/XMLSchema#nonNegativeInteger">1</owl:cardinality>
            </owl:Restriction>
        </rdfs:subClassOf>
        <rdfs:subClassOf>
            <owl:Restriction>
                <owl:onProperty rdf:resource="http://www.w3.org/ns/sosa/phenomenonTime"/>
                <owl:cardinality rdf:datatype="http://www.w3.org/2001/XMLSchema#nonNegativeInteger">1</owl:cardinality>
            </owl:Restriction>
        </rdfs:subClassOf>
        <rdfs:subClassOf>
            <owl:Restriction>
                <owl:onProperty rdf:resource="http://www.w3.org/ns/ssn/wasOriginatedBy"/>
                <owl:cardinality rdf:datatype="http://www.w3.org/2001/XMLSchema#nonNegativeInteger">1</owl:cardinality>
            </owl:Restriction>
        </rdfs:subClassOf>
        <rdfs:subClassOf>
            <owl:Restriction>
                <owl:onProperty rdf:resource="http://www.w3.org/ns/sosa/resultTime"/>
                <owl:cardinality rdf:datatype="http://www.w3.org/2001/XMLSchema#nonNegativeInteger">1</owl:cardinality>
            </owl:Restriction>
        </rdfs:subClassOf>
        <rdfs:isDefinedBy rdf:resource="http://www.w3.org/ns/sosa/"/>
    </owl:Class>
    


    <!-- http://www.w3.org/ns/sosa/Platform -->

    <rdf:Description rdf:about="http://www.w3.org/ns/sosa/Platform">
        <rdfs:subClassOf>
            <owl:Restriction>
                <owl:onProperty rdf:resource="http://www.w3.org/ns/sosa/hosts"/>
                <owl:allValuesFrom rdf:resource="http://www.w3.org/ns/ssn/System"/>
            </owl:Restriction>
        </rdfs:subClassOf>
        <rdfs:subClassOf>
            <owl:Restriction>
                <owl:onProperty rdf:resource="http://www.w3.org/ns/ssn/inDeployment"/>
                <owl:allValuesFrom rdf:resource="http://www.w3.org/ns/ssn/Deployment"/>
            </owl:Restriction>
        </rdfs:subClassOf>
        <rdfs:isDefinedBy rdf:resource="http://www.w3.org/ns/sosa/"/>
    </rdf:Description>
    


    <!-- http://www.w3.org/ns/sosa/Procedure -->

    <rdf:Description rdf:about="http://www.w3.org/ns/sosa/Procedure">
        <rdfs:subClassOf>
            <owl:Restriction>
                <owl:onProperty rdf:resource="http://www.w3.org/ns/ssn/hasInput"/>
                <owl:allValuesFrom rdf:resource="http://www.w3.org/ns/ssn/Input"/>
            </owl:Restriction>
        </rdfs:subClassOf>
        <rdfs:subClassOf>
            <owl:Restriction>
                <owl:onProperty rdf:resource="http://www.w3.org/ns/ssn/hasOutput"/>
                <owl:allValuesFrom rdf:resource="http://www.w3.org/ns/ssn/Output"/>
            </owl:Restriction>
        </rdfs:subClassOf>
        <rdfs:subClassOf>
            <owl:Restriction>
                <owl:onProperty rdf:resource="http://www.w3.org/ns/ssn/implementedBy"/>
                <owl:allValuesFrom rdf:resource="http://www.w3.org/ns/ssn/System"/>
            </owl:Restriction>
        </rdfs:subClassOf>
        <rdfs:isDefinedBy rdf:resource="http://www.w3.org/ns/sosa/"/>
    </rdf:Description>
    


    <!-- http://www.w3.org/ns/sosa/Result -->

    <rdf:Description rdf:about="http://www.w3.org/ns/sosa/Result">
        <rdfs:subClassOf>
            <owl:Restriction>
                <owl:onProperty rdf:resource="http://www.w3.org/ns/sosa/isResultOf"/>
                <owl:minCardinality rdf:datatype="http://www.w3.org/2001/XMLSchema#nonNegativeInteger">1</owl:minCardinality>
            </owl:Restriction>
        </rdfs:subClassOf>
        <rdfs:isDefinedBy rdf:resource="http://www.w3.org/ns/sosa/"/>
    </rdf:Description>
    


    <!-- http://www.w3.org/ns/sosa/Sample -->

    <rdf:Description rdf:about="http://www.w3.org/ns/sosa/Sample">
        <rdfs:subClassOf rdf:resource="http://www.w3.org/ns/sosa/FeatureOfInterest"/>
        <rdfs:subClassOf rdf:resource="http://www.w3.org/ns/sosa/Result"/>
        <rdfs:subClassOf>
            <owl:Restriction>
                <owl:onProperty rdf:resource="http://www.w3.org/ns/sosa/isResultOf"/>
                <owl:allValuesFrom rdf:resource="http://www.w3.org/ns/sosa/Sampling"/>
            </owl:Restriction>
        </rdfs:subClassOf>
        <rdfs:subClassOf>
            <owl:Restriction>
                <owl:onProperty rdf:resource="http://www.w3.org/ns/sosa/isSampleOf"/>
                <owl:allValuesFrom rdf:resource="http://www.w3.org/ns/sosa/FeatureOfInterest"/>
            </owl:Restriction>
        </rdfs:subClassOf>
        <rdfs:subClassOf>
            <owl:Restriction>
                <owl:onProperty rdf:resource="http://www.w3.org/ns/sosa/isResultOf"/>
                <owl:minCardinality rdf:datatype="http://www.w3.org/2001/XMLSchema#nonNegativeInteger">1</owl:minCardinality>
            </owl:Restriction>
        </rdfs:subClassOf>
        <rdfs:subClassOf>
            <owl:Restriction>
                <owl:onProperty rdf:resource="http://www.w3.org/ns/sosa/isSampleOf"/>
                <owl:minCardinality rdf:datatype="http://www.w3.org/2001/XMLSchema#nonNegativeInteger">1</owl:minCardinality>
            </owl:Restriction>
        </rdfs:subClassOf>
        <rdfs:isDefinedBy rdf:resource="http://www.w3.org/ns/sosa/"/>
    </rdf:Description>
    


    <!-- http://www.w3.org/ns/sosa/Sampler -->

    <rdf:Description rdf:about="http://www.w3.org/ns/sosa/Sampler">
        <rdfs:subClassOf rdf:resource="http://www.w3.org/ns/ssn/System"/>
        <rdfs:subClassOf>
            <owl:Restriction>
                <owl:onProperty rdf:resource="http://www.w3.org/ns/sosa/madeSampling"/>
                <owl:allValuesFrom rdf:resource="http://www.w3.org/ns/sosa/Sampling"/>
            </owl:Restriction>
        </rdfs:subClassOf>
        <rdfs:subClassOf>
            <owl:Restriction>
                <owl:onProperty rdf:resource="http://www.w3.org/ns/ssn/implements"/>
                <owl:minCardinality rdf:datatype="http://www.w3.org/2001/XMLSchema#nonNegativeInteger">1</owl:minCardinality>
            </owl:Restriction>
        </rdfs:subClassOf>
        <rdfs:isDefinedBy rdf:resource="http://www.w3.org/ns/sosa/"/>
    </rdf:Description>
    


    <!-- http://www.w3.org/ns/sosa/Sampling -->

    <owl:Class rdf:about="http://www.w3.org/ns/sosa/Sampling">
        <rdfs:subClassOf>
            <owl:Restriction>
                <owl:onProperty rdf:resource="http://www.w3.org/ns/sosa/hasFeatureOfInterest"/>
                <owl:allValuesFrom rdf:resource="http://www.w3.org/ns/sosa/FeatureOfInterest"/>
            </owl:Restriction>
        </rdfs:subClassOf>
        <rdfs:subClassOf>
            <owl:Restriction>
                <owl:onProperty rdf:resource="http://www.w3.org/ns/sosa/hasResult"/>
                <owl:allValuesFrom rdf:resource="http://www.w3.org/ns/sosa/Sample"/>
            </owl:Restriction>
        </rdfs:subClassOf>
        <rdfs:subClassOf>
            <owl:Restriction>
                <owl:onProperty rdf:resource="http://www.w3.org/ns/sosa/madeBySampler"/>
                <owl:allValuesFrom rdf:resource="http://www.w3.org/ns/sosa/Sampler"/>
            </owl:Restriction>
        </rdfs:subClassOf>
        <rdfs:subClassOf>
            <owl:Restriction>
                <owl:onProperty rdf:resource="http://www.w3.org/ns/sosa/usedProcedure"/>
                <owl:allValuesFrom rdf:resource="http://www.w3.org/ns/sosa/Procedure"/>
            </owl:Restriction>
        </rdfs:subClassOf>
        <rdfs:subClassOf>
            <owl:Restriction>
                <owl:onProperty rdf:resource="http://www.w3.org/ns/sosa/hasResult"/>
                <owl:minCardinality rdf:datatype="http://www.w3.org/2001/XMLSchema#nonNegativeInteger">1</owl:minCardinality>
            </owl:Restriction>
        </rdfs:subClassOf>
        <rdfs:subClassOf>
            <owl:Restriction>
                <owl:onProperty rdf:resource="http://www.w3.org/ns/sosa/hasFeatureOfInterest"/>
                <owl:cardinality rdf:datatype="http://www.w3.org/2001/XMLSchema#nonNegativeInteger">1</owl:cardinality>
            </owl:Restriction>
        </rdfs:subClassOf>
        <rdfs:subClassOf>
            <owl:Restriction>
                <owl:onProperty rdf:resource="http://www.w3.org/ns/sosa/madeBySampler"/>
                <owl:cardinality rdf:datatype="http://www.w3.org/2001/XMLSchema#nonNegativeInteger">1</owl:cardinality>
            </owl:Restriction>
        </rdfs:subClassOf>
        <rdfs:subClassOf>
            <owl:Restriction>
                <owl:onProperty rdf:resource="http://www.w3.org/ns/sosa/resultTime"/>
                <owl:cardinality rdf:datatype="http://www.w3.org/2001/XMLSchema#nonNegativeInteger">1</owl:cardinality>
            </owl:Restriction>
        </rdfs:subClassOf>
        <rdfs:isDefinedBy rdf:resource="http://www.w3.org/ns/sosa/"/>
    </owl:Class>
    


    <!-- http://www.w3.org/ns/sosa/Sensor -->

    <rdf:Description rdf:about="http://www.w3.org/ns/sosa/Sensor">
        <rdfs:subClassOf rdf:resource="http://www.w3.org/ns/ssn/System"/>
        <rdfs:subClassOf>
            <owl:Restriction>
                <owl:onProperty rdf:resource="http://www.w3.org/ns/sosa/madeObservation"/>
                <owl:allValuesFrom rdf:resource="http://www.w3.org/ns/sosa/Observation"/>
            </owl:Restriction>
        </rdfs:subClassOf>
        <rdfs:subClassOf>
            <owl:Restriction>
                <owl:onProperty rdf:resource="http://www.w3.org/ns/sosa/observes"/>
                <owl:allValuesFrom rdf:resource="http://www.w3.org/ns/sosa/ObservableProperty"/>
            </owl:Restriction>
        </rdfs:subClassOf>
        <rdfs:subClassOf>
            <owl:Restriction>
                <owl:onProperty rdf:resource="http://www.w3.org/ns/ssn/detects"/>
                <owl:allValuesFrom rdf:resource="http://www.w3.org/ns/ssn/Stimulus"/>
            </owl:Restriction>
        </rdfs:subClassOf>
        <rdfs:subClassOf>
            <owl:Restriction>
                <owl:onProperty rdf:resource="http://www.w3.org/ns/ssn/implements"/>
                <owl:minCardinality rdf:datatype="http://www.w3.org/2001/XMLSchema#nonNegativeInteger">1</owl:minCardinality>
            </owl:Restriction>
        </rdfs:subClassOf>
        <rdfs:isDefinedBy rdf:resource="http://www.w3.org/ns/sosa/"/>
    </rdf:Description>
    


    <!-- http://www.w3.org/ns/sosa/sampling/RelationshipNature -->

    <owl:Class rdf:about="http://www.w3.org/ns/sosa/sampling/RelationshipNature">
        <rdfs:comment>Nature of a relationship (between samples) - Members of this class indicate the nature of a relationship between two samples.</rdfs:comment>
        <rdfs:isDefinedBy>http://www.w3.org/ns/sosa/sampling/</rdfs:isDefinedBy>
    </owl:Class>
    


    <!-- http://www.w3.org/ns/sosa/sampling/SampleRelationship -->

    <owl:Class rdf:about="http://www.w3.org/ns/sosa/sampling/SampleRelationship">
        <rdfs:comment>Members of this class represent a relationship between a sample and another.</rdfs:comment>
        <rdfs:isDefinedBy>http://www.w3.org/ns/sosa/sampling/</rdfs:isDefinedBy>
    </owl:Class>
    


    <!-- http://www.w3.org/ns/ssn/Condition -->

    <owl:Class rdf:about="http://www.w3.org/ns/ssn/Condition">
        <rdfs:subClassOf rdf:resource="http://www.w3.org/ns/ssn/Property"/>
        <rdfs:comment>Used to specify ranges for qualities that act as Condition on a Systems&apos; operation.</rdfs:comment>
        <rdfs:isDefinedBy rdf:resource="http://www.w3.org/ns/sosa/"/>
        <rdfs:label>Condition</rdfs:label>
        <skos:example>For example, wind speed of 10-60m/s may be used as the Condition on a SystemProperty, for example, to state that a sensor has a particular Accuracy under that Condition.</skos:example>
    </owl:Class>
    


    <!-- http://www.w3.org/ns/ssn/Deployment -->

    <owl:Class rdf:about="http://www.w3.org/ns/ssn/Deployment">
        <rdfs:subClassOf>
            <owl:Restriction>
                <owl:onProperty rdf:resource="http://www.w3.org/ns/ssn/deployedOnPlatform"/>
                <owl:allValuesFrom rdf:resource="http://www.w3.org/ns/sosa/Platform"/>
            </owl:Restriction>
        </rdfs:subClassOf>
        <rdfs:subClassOf>
            <owl:Restriction>
                <owl:onProperty rdf:resource="http://www.w3.org/ns/ssn/deployedSystem"/>
                <owl:allValuesFrom rdf:resource="http://www.w3.org/ns/ssn/System"/>
            </owl:Restriction>
        </rdfs:subClassOf>
        <rdfs:subClassOf>
            <owl:Restriction>
                <owl:onProperty rdf:resource="http://www.w3.org/ns/ssn/forProperty"/>
                <owl:allValuesFrom rdf:resource="http://www.w3.org/ns/ssn/Property"/>
            </owl:Restriction>
        </rdfs:subClassOf>
        <rdfs:comment xml:lang="en">Describes the Deployment of one or more Systems for a particular purpose. Deployment may be done on a Platform.</rdfs:comment>
        <rdfs:isDefinedBy rdf:resource="http://www.w3.org/ns/ssn/"/>
        <rdfs:label xml:lang="en">Deployment</rdfs:label>
        <skos:definition xml:lang="en">Describes the Deployment of one or more Systems for a particular purpose. Deployment may be done on a Platform.</skos:definition>
        <skos:example xml:lang="en">For example, a temperature Sensor deployed on a wall, or a whole network of Sensors deployed for an Observation campaign.</skos:example>
    </owl:Class>
    


    <!-- http://www.w3.org/ns/ssn/Input -->

    <owl:Class rdf:about="http://www.w3.org/ns/ssn/Input">
        <rdfs:subClassOf>
            <owl:Restriction>
                <owl:onProperty>
                    <rdf:Description>
                        <owl:inverseOf rdf:resource="http://www.w3.org/ns/ssn/hasInput"/>
                    </rdf:Description>
                </owl:onProperty>
                <owl:allValuesFrom rdf:resource="http://www.w3.org/ns/sosa/Procedure"/>
            </owl:Restriction>
        </rdfs:subClassOf>
        <rdfs:subClassOf>
            <owl:Restriction>
                <owl:onProperty>
                    <rdf:Description>
                        <owl:inverseOf rdf:resource="http://www.w3.org/ns/ssn/hasInput"/>
                    </rdf:Description>
                </owl:onProperty>
                <owl:minCardinality rdf:datatype="http://www.w3.org/2001/XMLSchema#nonNegativeInteger">1</owl:minCardinality>
            </owl:Restriction>
        </rdfs:subClassOf>
        <rdfs:comment xml:lang="en">Any information that is provided to a Procedure for its use.</rdfs:comment>
        <rdfs:isDefinedBy rdf:resource="http://www.w3.org/ns/ssn/"/>
        <rdfs:label xml:lang="en">Input</rdfs:label>
        <skos:definition xml:lang="en">Any information that is provided to a Procedure for its use.</skos:definition>
    </owl:Class>
    


    <!-- http://www.w3.org/ns/ssn/Output -->

    <owl:Class rdf:about="http://www.w3.org/ns/ssn/Output">
        <rdfs:subClassOf>
            <owl:Restriction>
                <owl:onProperty>
                    <rdf:Description>
                        <owl:inverseOf rdf:resource="http://www.w3.org/ns/ssn/hasOutput"/>
                    </rdf:Description>
                </owl:onProperty>
                <owl:allValuesFrom rdf:resource="http://www.w3.org/ns/sosa/Procedure"/>
            </owl:Restriction>
        </rdfs:subClassOf>
        <rdfs:subClassOf>
            <owl:Restriction>
                <owl:onProperty>
                    <rdf:Description>
                        <owl:inverseOf rdf:resource="http://www.w3.org/ns/ssn/hasOutput"/>
                    </rdf:Description>
                </owl:onProperty>
                <owl:minCardinality rdf:datatype="http://www.w3.org/2001/XMLSchema#nonNegativeInteger">1</owl:minCardinality>
            </owl:Restriction>
        </rdfs:subClassOf>
        <rdfs:comment xml:lang="en">Any information that is reported from a Procedure.</rdfs:comment>
        <rdfs:isDefinedBy rdf:resource="http://www.w3.org/ns/ssn/"/>
        <rdfs:label xml:lang="en">Output</rdfs:label>
        <skos:definition xml:lang="en">Any information that is reported from a Procedure.</skos:definition>
    </owl:Class>
    


    <!-- http://www.w3.org/ns/ssn/OversamplingRate -->

    <owl:Class rdf:about="http://www.w3.org/ns/ssn/OversamplingRate">
        <rdfs:subClassOf rdf:resource="http://www.w3.org/ns/ssn/systems/SystemProperty"/>
        <rdfs:comment>Specifies the number of sensor measurements used internally to generate one sensor output result. (Oversampling rate = OSR)</rdfs:comment>
        <rdfs:label>Oversampling Rate</rdfs:label>
    </owl:Class>
    


    <!-- http://www.w3.org/ns/ssn/Property -->

    <owl:Class rdf:about="http://www.w3.org/ns/ssn/Property">
        <rdfs:subClassOf>
            <owl:Restriction>
                <owl:onProperty rdf:resource="http://www.w3.org/ns/ssn/isPropertyOf"/>
                <owl:allValuesFrom rdf:resource="http://www.w3.org/ns/sosa/FeatureOfInterest"/>
            </owl:Restriction>
        </rdfs:subClassOf>
        <rdfs:comment xml:lang="en">A quality of an entity. An aspect of an entity that is intrinsic to and cannot exist without the entity.</rdfs:comment>
        <rdfs:isDefinedBy rdf:resource="http://www.w3.org/ns/ssn/"/>
        <rdfs:label xml:lang="en">Property</rdfs:label>
        <skos:definition xml:lang="en">A quality of an entity. An aspect of an entity that is intrinsic to and cannot exist without the entity.</skos:definition>
    </owl:Class>
    


    <!-- http://www.w3.org/ns/ssn/Stimulus -->

    <owl:Class rdf:about="http://www.w3.org/ns/ssn/Stimulus">
        <rdfs:subClassOf>
            <owl:Restriction>
                <owl:onProperty rdf:resource="http://www.w3.org/ns/ssn/isProxyFor"/>
                <owl:allValuesFrom rdf:resource="http://www.w3.org/ns/sosa/ObservableProperty"/>
            </owl:Restriction>
        </rdfs:subClassOf>
        <rdfs:subClassOf>
            <owl:Restriction>
                <owl:onProperty>
                    <rdf:Description>
                        <owl:inverseOf rdf:resource="http://www.w3.org/ns/ssn/detects"/>
                    </rdf:Description>
                </owl:onProperty>
                <owl:allValuesFrom rdf:resource="http://www.w3.org/ns/sosa/Sensor"/>
            </owl:Restriction>
        </rdfs:subClassOf>
        <rdfs:subClassOf>
            <owl:Restriction>
                <owl:onProperty>
                    <rdf:Description>
                        <owl:inverseOf rdf:resource="http://www.w3.org/ns/ssn/wasOriginatedBy"/>
                    </rdf:Description>
                </owl:onProperty>
                <owl:allValuesFrom rdf:resource="http://www.w3.org/ns/sosa/Observation"/>
            </owl:Restriction>
        </rdfs:subClassOf>
        <rdfs:comment xml:lang="en">An event in the real world that &apos;triggers&apos; the Sensor. The properties associated to the Stimulus may be different to the eventual observed ObservableProperty. It is the event, not the object, that triggers the Sensor.</rdfs:comment>
        <rdfs:isDefinedBy rdf:resource="http://www.w3.org/ns/ssn/"/>
        <rdfs:label xml:lang="en">Stimulus</rdfs:label>
        <skos:definition xml:lang="en">An event in the real world that &apos;triggers&apos; the Sensor. The properties associated to the Stimulus may be different to the eventual observed ObservableProperty. It is the event, not the object, that triggers the Sensor.</skos:definition>
    </owl:Class>
    


    <!-- http://www.w3.org/ns/ssn/System -->

    <owl:Class rdf:about="http://www.w3.org/ns/ssn/System">
        <rdfs:subClassOf>
            <owl:Restriction>
                <owl:onProperty rdf:resource="http://www.w3.org/ns/sosa/isHostedBy"/>
                <owl:allValuesFrom rdf:resource="http://www.w3.org/ns/sosa/Platform"/>
            </owl:Restriction>
        </rdfs:subClassOf>
        <rdfs:subClassOf>
            <owl:Restriction>
                <owl:onProperty rdf:resource="http://www.w3.org/ns/ssn/hasDeployment"/>
                <owl:allValuesFrom rdf:resource="http://www.w3.org/ns/ssn/Deployment"/>
            </owl:Restriction>
        </rdfs:subClassOf>
        <rdfs:subClassOf>
            <owl:Restriction>
                <owl:onProperty rdf:resource="http://www.w3.org/ns/ssn/hasSubSystem"/>
                <owl:allValuesFrom rdf:resource="http://www.w3.org/ns/ssn/System"/>
            </owl:Restriction>
        </rdfs:subClassOf>
        <rdfs:subClassOf>
            <owl:Restriction>
                <owl:onProperty rdf:resource="http://www.w3.org/ns/ssn/implements"/>
                <owl:allValuesFrom rdf:resource="http://www.w3.org/ns/sosa/Procedure"/>
            </owl:Restriction>
        </rdfs:subClassOf>
        <rdfs:subClassOf>
            <owl:Restriction>
                <owl:onProperty>
                    <rdf:Description>
                        <owl:inverseOf rdf:resource="http://www.w3.org/ns/ssn/hasSubSystem"/>
                    </rdf:Description>
                </owl:onProperty>
                <owl:allValuesFrom rdf:resource="http://www.w3.org/ns/ssn/System"/>
            </owl:Restriction>
        </rdfs:subClassOf>
        <rdfs:comment xml:lang="en">System is a unit of abstraction for pieces of infrastructure that implement Procedures. A System may have components, its subsystems, which are other systems.</rdfs:comment>
        <rdfs:isDefinedBy rdf:resource="http://www.w3.org/ns/ssn/"/>
        <rdfs:label xml:lang="en">System</rdfs:label>
        <skos:definition xml:lang="en">System is a unit of abstraction for pieces of infrastructure that implement Procedures. A System may have components, its subsystems, which are other systems.</skos:definition>
    </owl:Class>
    


    <!-- http://www.w3.org/ns/ssn/systems/Accuracy -->

    <owl:Class rdf:about="http://www.w3.org/ns/ssn/systems/Accuracy">
        <rdfs:subClassOf rdf:resource="http://www.w3.org/ns/ssn/systems/SystemProperty"/>
        <rdfs:comment>The closeness of agreement between the Result of an Observation (resp. The command of an Actuation) and the true value of the observed ObservableProperty (resp. Of the acted on ActuableProperty) under the defined Conditions.</rdfs:comment>
        <rdfs:isDefinedBy rdf:resource="http://www.w3.org/ns/sosa/"/>
        <rdfs:label>Accuracy</rdfs:label>
    </owl:Class>
    


    <!-- http://www.w3.org/ns/ssn/systems/ActuationRange -->

    <owl:Class rdf:about="http://www.w3.org/ns/ssn/systems/ActuationRange">
        <rdfs:subClassOf rdf:resource="http://www.w3.org/ns/ssn/systems/SystemProperty"/>
        <rdfs:comment>The range of property values that can be the Result of an Actuation under the defined Conditions.</rdfs:comment>
        <rdfs:isDefinedBy rdf:resource="http://www.w3.org/ns/sosa/"/>
        <rdfs:label>Actuation Range</rdfs:label>
    </owl:Class>
    


    <!-- http://www.w3.org/ns/ssn/systems/BatteryLifetime -->

    <owl:Class rdf:about="http://www.w3.org/ns/ssn/systems/BatteryLifetime">
        <rdfs:subClassOf rdf:resource="http://www.w3.org/ns/ssn/systems/SurvivalProperty"/>
        <rdfs:comment>Total useful life of a System&apos;s battery in the specified Conditions.</rdfs:comment>
        <rdfs:isDefinedBy rdf:resource="http://www.w3.org/ns/sosa/"/>
        <rdfs:label>Battery Lifetime</rdfs:label>
    </owl:Class>
    


    <!-- http://www.w3.org/ns/ssn/systems/DetectionLimit -->

    <owl:Class rdf:about="http://www.w3.org/ns/ssn/systems/DetectionLimit">
        <rdfs:subClassOf rdf:resource="http://www.w3.org/ns/ssn/systems/SystemProperty"/>
        <rdfs:comment>An observed value for which the probability of falsely claiming the absence of a component in a material is beta, given a probability alpha of falsely claiming its presence.</rdfs:comment>
        <rdfs:isDefinedBy rdf:resource="http://www.w3.org/ns/sosa/"/>
        <rdfs:label>Detection Limit</rdfs:label>
    </owl:Class>
    


    <!-- http://www.w3.org/ns/ssn/systems/Drift -->

    <owl:Class rdf:about="http://www.w3.org/ns/ssn/systems/Drift">
        <rdfs:subClassOf rdf:resource="http://www.w3.org/ns/ssn/systems/SystemProperty"/>
        <rdfs:comment>As a Sensor Property: a continuous or incremental change in the reported values of Observations over time for an unchanging Property under the defined Conditions. As an Actuator Property: a continuous or incremental change in the true value of the acted on ActuableProperty over time for an unchanging command under the defined Conditions.</rdfs:comment>
        <rdfs:isDefinedBy rdf:resource="http://www.w3.org/ns/sosa/"/>
        <rdfs:label>Drift</rdfs:label>
    </owl:Class>
    


    <!-- http://www.w3.org/ns/ssn/systems/Frequency -->

    <owl:Class rdf:about="http://www.w3.org/ns/ssn/systems/Frequency">
        <rdfs:subClassOf rdf:resource="http://www.w3.org/ns/ssn/systems/SystemProperty"/>
        <rdfs:comment>The smallest possible time between one Observation, Actuation, or Sampling and the next, under the defined Conditions.</rdfs:comment>
        <rdfs:isDefinedBy rdf:resource="http://www.w3.org/ns/sosa/"/>
        <rdfs:label>Frequency</rdfs:label>
    </owl:Class>
    


    <!-- http://www.w3.org/ns/ssn/systems/Latency -->

    <owl:Class rdf:about="http://www.w3.org/ns/ssn/systems/Latency">
        <rdfs:subClassOf rdf:resource="http://www.w3.org/ns/ssn/systems/SystemProperty"/>
        <rdfs:comment>The time between a command for an Observation and the Sensor providing a Result, under the defined Conditions.</rdfs:comment>
        <rdfs:isDefinedBy rdf:resource="http://www.w3.org/ns/sosa/"/>
        <rdfs:label>Latency</rdfs:label>
    </owl:Class>
    


    <!-- http://www.w3.org/ns/ssn/systems/MaintenanceSchedule -->

    <owl:Class rdf:about="http://www.w3.org/ns/ssn/systems/MaintenanceSchedule">
        <rdfs:subClassOf rdf:resource="http://www.w3.org/ns/ssn/systems/OperatingProperty"/>
        <rdfs:comment>Schedule of maintenance for a System in the specified Conditions.</rdfs:comment>
        <rdfs:isDefinedBy rdf:resource="http://www.w3.org/ns/sosa/"/>
        <rdfs:label>Maintenance Schdule</rdfs:label>
    </owl:Class>
    


    <!-- http://www.w3.org/ns/ssn/systems/MeasurementRange -->

    <owl:Class rdf:about="http://www.w3.org/ns/ssn/systems/MeasurementRange">
        <rdfs:subClassOf rdf:resource="http://www.w3.org/ns/ssn/systems/SystemProperty"/>
        <rdfs:comment>The set of values that the Sensor can return as the Result of an Observation under the defined Conditions with the defined system properties.</rdfs:comment>
        <rdfs:isDefinedBy rdf:resource="http://www.w3.org/ns/sosa/"/>
        <rdfs:label>Measurement Range</rdfs:label>
    </owl:Class>
    


    <!-- http://www.w3.org/ns/ssn/systems/OperatingPowerRange -->

    <owl:Class rdf:about="http://www.w3.org/ns/ssn/systems/OperatingPowerRange">
        <rdfs:subClassOf rdf:resource="http://www.w3.org/ns/ssn/systems/OperatingProperty"/>
        <rdfs:comment>Power range in which System is expected to operate in the specified.</rdfs:comment>
        <rdfs:isDefinedBy rdf:resource="http://www.w3.org/ns/sosa/"/>
        <rdfs:label>Operating Power Range</rdfs:label>
    </owl:Class>
    


    <!-- http://www.w3.org/ns/ssn/systems/OperatingProperty -->

    <owl:Class rdf:about="http://www.w3.org/ns/ssn/systems/OperatingProperty">
        <rdfs:subClassOf rdf:resource="http://www.w3.org/ns/ssn/Property"/>
        <rdfs:comment>An identifiable characteristic that represents how the System operates under the specified Conditions. May describe power ranges, power sources, standard configurations, attachments and the like.</rdfs:comment>
        <rdfs:isDefinedBy rdf:resource="http://www.w3.org/ns/sosa/"/>
        <rdfs:label>Operating Property</rdfs:label>
    </owl:Class>
    


    <!-- http://www.w3.org/ns/ssn/systems/OperatingRange -->

    <owl:Class rdf:about="http://www.w3.org/ns/ssn/systems/OperatingRange">
        <rdfs:subClassOf rdf:resource="http://www.w3.org/ns/ssn/Property"/>
        <rdfs:comment>&quot;Describes normal OperatingProperties of a System under some specified Conditions. For example, to the power requirement or maintenance schedule of a System under a specified temperature range.
In the absence of OperatingProperties, it simply describes the Conditions in which a System is expected to operate.&quot;</rdfs:comment>
        <rdfs:isDefinedBy rdf:resource="http://www.w3.org/ns/sosa/"/>
        <rdfs:label>Operating Range</rdfs:label>
    </owl:Class>
    


    <!-- http://www.w3.org/ns/ssn/systems/Precision -->

    <owl:Class rdf:about="http://www.w3.org/ns/ssn/systems/Precision">
        <rdfs:subClassOf rdf:resource="http://www.w3.org/ns/ssn/systems/SystemProperty"/>
        <rdfs:comment>As a sensor capability: The closeness of agreement between replicate Observations on an unchanged or similar quality value: i.e., a measure of a Sensor&apos;s ability to consistently reproduce an Observation, under the defined Conditions.</rdfs:comment>
        <rdfs:isDefinedBy rdf:resource="http://www.w3.org/ns/sosa/"/>
        <rdfs:label>Precision</rdfs:label>
    </owl:Class>
    


    <!-- http://www.w3.org/ns/ssn/systems/Resolution -->

    <owl:Class rdf:about="http://www.w3.org/ns/ssn/systems/Resolution">
        <rdfs:subClassOf rdf:resource="http://www.w3.org/ns/ssn/systems/SystemProperty"/>
        <rdfs:comment>As an actuator capability: The closeness of agreement between replicate Actuations for an unchanged or similar command: i.e., a measure of an Actuator&apos;s ability to consistently reproduce an Actuations, under the defined Conditions.</rdfs:comment>
        <rdfs:isDefinedBy rdf:resource="http://www.w3.org/ns/sosa/"/>
        <rdfs:label>Resolution</rdfs:label>
    </owl:Class>
    


    <!-- http://www.w3.org/ns/ssn/systems/ResponseTime -->

    <owl:Class rdf:about="http://www.w3.org/ns/ssn/systems/ResponseTime">
        <rdfs:subClassOf rdf:resource="http://www.w3.org/ns/ssn/systems/SystemProperty"/>
        <rdfs:comment>As a Sensor Property: the time between a (step) change in the value of an observed ObservableProperty and a Sensor (possibly with specified error) &apos;settling&apos; on an observed value, under the defined Conditions.</rdfs:comment>
        <rdfs:isDefinedBy rdf:resource="http://www.w3.org/ns/sosa/"/>
        <rdfs:label>Response Time</rdfs:label>
    </owl:Class>
    


    <!-- http://www.w3.org/ns/ssn/systems/Selectivity -->

    <owl:Class rdf:about="http://www.w3.org/ns/ssn/systems/Selectivity">
        <rdfs:subClassOf rdf:resource="http://www.w3.org/ns/ssn/systems/SystemProperty"/>
        <rdfs:comment>As an Actuator Property: the time between a (step) change in the command of an Actuator and the &apos;settling&apos; of the value of the acted on ActuatableProperty, under the defined Conditions.</rdfs:comment>
        <rdfs:isDefinedBy rdf:resource="http://www.w3.org/ns/sosa/"/>
        <rdfs:label>Selectivity</rdfs:label>
    </owl:Class>
    


    <!-- http://www.w3.org/ns/ssn/systems/Sensitivity -->

    <owl:Class rdf:about="http://www.w3.org/ns/ssn/systems/Sensitivity">
        <rdfs:subClassOf rdf:resource="http://www.w3.org/ns/ssn/systems/SystemProperty"/>
        <rdfs:comment>As a Sensor Property: Sensitivity is the quotient of the change in a Result of Observations and the corresponding change in a value of an ObservableProperty being observed, under the defined Conditions.</rdfs:comment>
        <rdfs:isDefinedBy rdf:resource="http://www.w3.org/ns/sosa/"/>
        <rdfs:label>Sensitivity</rdfs:label>
    </owl:Class>
    


    <!-- http://www.w3.org/ns/ssn/systems/SurvivalProperty -->

    <owl:Class rdf:about="http://www.w3.org/ns/ssn/systems/SurvivalProperty">
        <rdfs:subClassOf rdf:resource="http://www.w3.org/ns/ssn/Property"/>
        <rdfs:comment>An identifiable characteristic that represents the extent of the System&apos;s useful life under the specified Conditions. May describe for example total battery life or number of recharges, or, for Sensors that are used only a fixed number of times, the number of Observations that can be made before the sensing capability is depleted.</rdfs:comment>
        <rdfs:isDefinedBy rdf:resource="http://www.w3.org/ns/sosa/"/>
        <rdfs:label>Survival Property</rdfs:label>
    </owl:Class>
    


    <!-- http://www.w3.org/ns/ssn/systems/SurvivalRange -->

    <owl:Class rdf:about="http://www.w3.org/ns/ssn/systems/SurvivalRange">
        <rdfs:subClassOf rdf:resource="http://www.w3.org/ns/ssn/Property"/>
        <rdfs:comment>&quot;Describes SurvivalProperties of a System under some specified Conditions. For example, the lifetime of a System under a specified temperature range.
In the absence of SurvivalProperties, simply describes the Conditions a System can be exposed to without damage. For example, the temperature range a System can withstand before being considered damaged.&quot;</rdfs:comment>
        <rdfs:isDefinedBy rdf:resource="http://www.w3.org/ns/sosa/"/>
        <rdfs:label>Survival Range</rdfs:label>
    </owl:Class>
    


    <!-- http://www.w3.org/ns/ssn/systems/SystemCapability -->

    <owl:Class rdf:about="http://www.w3.org/ns/ssn/systems/SystemCapability">
        <rdfs:subClassOf rdf:resource="http://www.w3.org/ns/ssn/Property"/>
        <rdfs:subClassOf>
            <owl:Restriction>
                <owl:onProperty rdf:resource="http://www.w3.org/ns/ssn/forProperty"/>
                <owl:allValuesFrom rdf:resource="http://www.w3.org/ns/ssn/Property"/>
            </owl:Restriction>
        </rdfs:subClassOf>
        <rdfs:comment>Describes normal measurement, actuation, sampling properties such as accuracy, range, precision, etc. Of a System under some specified Conditions such as temperature range. The capabilities specified here are those that affect the primary purpose of the System, while those in OperatingRange represent the system&apos;s normal operating environment, including Conditions that don&apos;t affect the Observations or the Actuations.</rdfs:comment>
        <rdfs:isDefinedBy rdf:resource="http://www.w3.org/ns/sosa/"/>
        <rdfs:label>System Capability</rdfs:label>
    </owl:Class>
    


    <!-- http://www.w3.org/ns/ssn/systems/SystemLifetime -->

    <owl:Class rdf:about="http://www.w3.org/ns/ssn/systems/SystemLifetime">
        <rdfs:subClassOf rdf:resource="http://www.w3.org/ns/ssn/systems/SurvivalProperty"/>
        <rdfs:comment>The System continues to operate as defined using SystemCapability. If, however, the SurvivalRange is violated, the System is &apos;damaged&apos; and SystemCapability specifications may no longer hold.</rdfs:comment>
        <rdfs:isDefinedBy rdf:resource="http://www.w3.org/ns/sosa/"/>
        <rdfs:label>System Lifetime</rdfs:label>
    </owl:Class>
    


    <!-- http://www.w3.org/ns/ssn/systems/SystemProperty -->

    <owl:Class rdf:about="http://www.w3.org/ns/ssn/systems/SystemProperty">
        <rdfs:subClassOf rdf:resource="http://www.w3.org/ns/ssn/Property"/>
        <rdfs:comment>An identifiable and observable characteristic that represents the system&apos;s ability to operate its primary purpose: a sensor to make Observations, an Actuator to make Actuations, or a Sampler to make Sampling.</rdfs:comment>
        <rdfs:isDefinedBy rdf:resource="http://www.w3.org/ns/sosa/"/>
        <rdfs:label>System Property</rdfs:label>
    </owl:Class>
    


    <!-- http://xmlns.com/foaf/0.1/Agent -->

    <owl:Class rdf:about="http://xmlns.com/foaf/0.1/Agent">
        <rdfs:comment>&quot;The Agent class is the class of agents; things that do stuff. A well known sub-class is Person, representing people. Other kinds of agents include Organization and Group.

The Agent class is useful in a few places in FOAF where Person would have been overly specific. For example, the IM chat ID properties such as jabberID are typically associated with people, but sometimes belong to software bots.&quot;</rdfs:comment>
        <rdfs:label>Agent</rdfs:label>
    </owl:Class>
    


    <!-- 
    ///////////////////////////////////////////////////////////////////////////////////////
    //
    // Individuals
    //
    ///////////////////////////////////////////////////////////////////////////////////////
     -->

    


    <!-- http://www.w3.org/ns/ssn/ -->

    <owl:NamedIndividual rdf:about="http://www.w3.org/ns/ssn/">
        <rdf:type rdf:resource="http://purl.org/vocommons/voaf#Vocabulary"/>
    </owl:NamedIndividual>
    


    <!-- http://www.w3.org/ns/ssn/systems/ -->

    <owl:NamedIndividual rdf:about="http://www.w3.org/ns/ssn/systems/"/>
    <rdf:Description>
        <rdf:type rdf:resource="http://xmlns.com/foaf/0.1/Agent"/>
        <foaf:name xml:lang="en">W3C/OGC Spatial Data on the Web Working Group</foaf:name>
    </rdf:Description>
    <rdf:Description>
        <rdf:type rdf:resource="http://xmlns.com/foaf/0.1/Agent"/>
        <foaf:name xml:lang="en">W3C/OGC Spatial Data on the Web Working Group</foaf:name>
    </rdf:Description>
    <rdf:Description>
        <rdf:type rdf:resource="http://xmlns.com/foaf/0.1/Agent"/>
        <foaf:name xml:lang="en">W3C/OGC Spatial Data on the Web Working Group</foaf:name>
    </rdf:Description>
    <rdf:Description>
        <rdf:type rdf:resource="http://xmlns.com/foaf/0.1/Agent"/>
        <foaf:name xml:lang="en">W3C/OGC Spatial Data on the Web Working Group</foaf:name>
    </rdf:Description>
    <rdf:Description>
        <rdf:type rdf:resource="http://xmlns.com/foaf/0.1/Agent"/>
        <foaf:name xml:lang="en">W3C/OGC Spatial Data on the Web Working Group</foaf:name>
    </rdf:Description>
    <rdf:Description>
        <rdf:type rdf:resource="http://xmlns.com/foaf/0.1/Agent"/>
        <foaf:name xml:lang="en">W3C/OGC Spatial Data on the Web Working Group</foaf:name>
    </rdf:Description>
    <rdf:Description>
        <rdf:type rdf:resource="http://xmlns.com/foaf/0.1/Agent"/>
        <foaf:name xml:lang="en">W3C/OGC Spatial Data on the Web Working Group</foaf:name>
    </rdf:Description>
    <rdf:Description>
        <rdf:type rdf:resource="http://xmlns.com/foaf/0.1/Agent"/>
        <foaf:name xml:lang="en">W3C/OGC Spatial Data on the Web Working Group</foaf:name>
    </rdf:Description>
    


    <!-- 
    ///////////////////////////////////////////////////////////////////////////////////////
    //
    // Annotations
    //
    ///////////////////////////////////////////////////////////////////////////////////////
     -->

    <rdf:Description rdf:about="http://www.w3.org/ns/sosa/hasSimpleResult">
        <rdfs:isDefinedBy rdf:resource="http://www.w3.org/ns/sosa/"/>
    </rdf:Description>
</rdf:RDF>



<!-- Generated by the OWL API (version 4.5.26.2023-07-17T20:34:13Z) https://github.com/owlcs/owlapi -->

